replace subexp definition with bind analysis as part of flow analysis

Abstract_Value_Flow_Analysis.thy
@@ -5,102 +5,118 @@ begin
 datatype abstract_value = A_Chan var ("^Chan _" [61] 61) | A_Unit ("^\<lparr>\<rparr>") | A_Prim prim ("^_" [61] 61 )
 
 type_synonym abstract_value_env = "var \<Rightarrow> abstract_value set"
-
+type_synonym bind_env = "var \<Rightarrow> bind set"
 fun result_var :: "exp \<Rightarrow> var" ("\<lfloor>_\<rfloor>" [0]61) where
   "\<lfloor>RESULT x\<rfloor> = x" |
   "\<lfloor>LET _ = _ in e\<rfloor> = \<lfloor>e\<rfloor>"
 
 
-inductive accept_exp :: "abstract_value_env \<times> abstract_value_env \<Rightarrow> exp \<Rightarrow> bool" (infix "\<Turnstile>\<^sub>e" 55) where
+inductive accept_exp :: "abstract_value_env \<times> abstract_value_env \<times> bind_env \<Rightarrow> exp \<Rightarrow> bool" (infix "\<Turnstile>\<^sub>e" 55) where
   "
-    (\<V>, \<C>) \<Turnstile>\<^sub>e (RESULT x)
+    (\<V>, \<C>, \<X>) \<Turnstile>\<^sub>e (RESULT x)
   " |
   Let_Unit: "
-    \<lbrakk> {^\<lparr>\<rparr>} \<subseteq> \<V> x; (\<V>, \<C>) \<Turnstile>\<^sub>e e \<rbrakk> \<Longrightarrow> 
-    (\<V>, \<C>) \<Turnstile>\<^sub>e LET x = \<lparr>\<rparr> in e
+    \<lbrakk> 
+      {\<lparr>\<rparr>} \<subseteq> \<X> x;
+      {^\<lparr>\<rparr>} \<subseteq> \<V> x; 
+      (\<V>, \<C>, \<X>) \<Turnstile>\<^sub>e e 
+    \<rbrakk> \<Longrightarrow> 
+    (\<V>, \<C>, \<X>) \<Turnstile>\<^sub>e LET x = \<lparr>\<rparr> in e
   " |
   Let_Abs : "
     \<lbrakk> 
+      {FN f' x' . e' } \<subseteq> \<X> f';
       {^Abs f' x' e'} \<subseteq> \<V> f';
-      (\<V>, \<C>) \<Turnstile>\<^sub>e e';
+      (\<V>, \<C>, \<X>) \<Turnstile>\<^sub>e e';
+      {FN f' x' . e' } \<subseteq> \<X> x;
       {^Abs f' x' e'} \<subseteq> \<V> x;
-      (\<V>, \<C>) \<Turnstile>\<^sub>e e 
+      (\<V>, \<C>, \<X>) \<Turnstile>\<^sub>e e 
     \<rbrakk> \<Longrightarrow> 
-    (\<V>, \<C>) \<Turnstile>\<^sub>e LET x = FN f' x' . e' in e
+    (\<V>, \<C>, \<X>) \<Turnstile>\<^sub>e LET x = FN f' x' . e' in e
   " |
   Let_Pair : "
     \<lbrakk> 
+      {\<lparr>x\<^sub>1, x\<^sub>2\<rparr>} \<subseteq> \<X> x;
       {^Pair x\<^sub>1 x\<^sub>2} \<subseteq> \<V> x;
-      (\<V>, \<C>) \<Turnstile>\<^sub>e e 
+      (\<V>, \<C>, \<X>) \<Turnstile>\<^sub>e e 
     \<rbrakk> \<Longrightarrow> 
-    (\<V>, \<C>) \<Turnstile>\<^sub>e LET x = \<lparr>x\<^sub>1, x\<^sub>2\<rparr> in e
+    (\<V>, \<C>, \<X>) \<Turnstile>\<^sub>e LET x = \<lparr>x\<^sub>1, x\<^sub>2\<rparr> in e
   " |
   Let_Left : "
     \<lbrakk> 
+      {LEFT x\<^sub>p} \<subseteq> \<X> x;
       {^Left x\<^sub>p} \<subseteq> \<V> x;
-      (\<V>, \<C>) \<Turnstile>\<^sub>e e 
+      (\<V>, \<C>, \<X>) \<Turnstile>\<^sub>e e 
     \<rbrakk> \<Longrightarrow> 
-    (\<V>, \<C>) \<Turnstile>\<^sub>e LET x = LEFT x\<^sub>p in e
+    (\<V>, \<C>, \<X>) \<Turnstile>\<^sub>e LET x = LEFT x\<^sub>p in e
   " |
   Let_Right : "
     \<lbrakk>
+      {RIGHT x\<^sub>p} \<subseteq> \<X> x;
       {^Right x\<^sub>p} \<subseteq> \<V> x;
-      (\<V>, \<C>) \<Turnstile>\<^sub>e e
+      (\<V>, \<C>, \<X>) \<Turnstile>\<^sub>e e
     \<rbrakk> \<Longrightarrow> 
-    (\<V>, \<C>) \<Turnstile>\<^sub>e LET x = RIGHT x\<^sub>p in e
+    (\<V>, \<C>, \<X>) \<Turnstile>\<^sub>e LET x = RIGHT x\<^sub>p in e
   " |
   Let_Send_Evt : "
     \<lbrakk> 
+      {SEND EVT x\<^sub>c x\<^sub>m} \<subseteq> \<X> x;
       {^Send_Evt x\<^sub>c x\<^sub>m} \<subseteq> \<V> x;
-      (\<V>, \<C>) \<Turnstile>\<^sub>e e 
+      (\<V>, \<C>, \<X>) \<Turnstile>\<^sub>e e 
     \<rbrakk> \<Longrightarrow> 
-    (\<V>, \<C>) \<Turnstile>\<^sub>e LET x = SEND EVT x\<^sub>c x\<^sub>m in e
+    (\<V>, \<C>, \<X>) \<Turnstile>\<^sub>e LET x = SEND EVT x\<^sub>c x\<^sub>m in e
   " |
   Let_Recv_Evt : "
     \<lbrakk> 
+      {RECV EVT x\<^sub>c} \<subseteq> \<X> x;
       {^Recv_Evt x\<^sub>c} \<subseteq> \<V> x;
-      (\<V>, \<C>) \<Turnstile>\<^sub>e e 
+      (\<V>, \<C>, \<X>) \<Turnstile>\<^sub>e e 
     \<rbrakk> \<Longrightarrow> 
-    (\<V>, \<C>) \<Turnstile>\<^sub>e LET x = RECV EVT x\<^sub>c in e
+    (\<V>, \<C>, \<X>) \<Turnstile>\<^sub>e LET x = RECV EVT x\<^sub>c in e
   " |
   Let_Case: "
     \<lbrakk>
-      \<forall> x\<^sub>l' . ^Left x\<^sub>l' \<in> \<V> x\<^sub>s \<longrightarrow> 
-        \<V> x\<^sub>l' \<subseteq> \<V> x\<^sub>l \<and> \<V> (\<lfloor>e\<^sub>l\<rfloor>) \<subseteq> \<V> x \<and> (\<V>, \<C>) \<Turnstile>\<^sub>e e\<^sub>l
+      {CASE x\<^sub>s LEFT x\<^sub>l |> e\<^sub>l RIGHT x\<^sub>r |> e\<^sub>r} \<subseteq> \<X> x;
+      \<forall> x\<^sub>l' . ^Left x\<^sub>l' \<in> \<V> x\<^sub>s \<longrightarrow>
+        \<V> x\<^sub>l' \<subseteq> \<V> x\<^sub>l \<and> \<V> (\<lfloor>e\<^sub>l\<rfloor>) \<subseteq> \<V> x \<and> (\<V>, \<C>, \<X>) \<Turnstile>\<^sub>e e\<^sub>l
       ;
       \<forall> x\<^sub>r' . ^Right x\<^sub>r' \<in> \<V> x\<^sub>s \<longrightarrow>
-        \<V> x\<^sub>r' \<subseteq> \<V> x\<^sub>r \<and> \<V> (\<lfloor>e\<^sub>r\<rfloor>) \<subseteq> \<V> x \<and> (\<V>, \<C>) \<Turnstile>\<^sub>e e\<^sub>r
+        \<V> x\<^sub>r' \<subseteq> \<V> x\<^sub>r \<and> \<V> (\<lfloor>e\<^sub>r\<rfloor>) \<subseteq> \<V> x \<and> (\<V>, \<C>, \<X>) \<Turnstile>\<^sub>e e\<^sub>r
       ;
-      (\<V>, \<C>) \<Turnstile>\<^sub>e e
+      (\<V>, \<C>, \<X>) \<Turnstile>\<^sub>e e
     \<rbrakk> \<Longrightarrow> 
-    (\<V>, \<C>) \<Turnstile>\<^sub>e LET x = CASE x\<^sub>s LEFT x\<^sub>l |> e\<^sub>l RIGHT x\<^sub>r |> e\<^sub>r in e
+    (\<V>, \<C>, \<X>) \<Turnstile>\<^sub>e LET x = CASE x\<^sub>s LEFT x\<^sub>l |> e\<^sub>l RIGHT x\<^sub>r |> e\<^sub>r in e
   " |
   Let_Fst: "
     \<lbrakk> 
+      {FST x\<^sub>p} \<subseteq> \<X> x;
       \<forall> x\<^sub>1 x\<^sub>2. ^Pair x\<^sub>1 x\<^sub>2 \<in> \<V> x\<^sub>p \<longrightarrow> \<V> x\<^sub>1 \<subseteq> \<V> x; 
-      (\<V>, \<C>) \<Turnstile>\<^sub>e e 
+      (\<V>, \<C>, \<X>) \<Turnstile>\<^sub>e e 
     \<rbrakk> \<Longrightarrow> 
-    (\<V>, \<C>) \<Turnstile>\<^sub>e LET x = FST x\<^sub>p in e
+    (\<V>, \<C>, \<X>) \<Turnstile>\<^sub>e LET x = FST x\<^sub>p in e
   " |
   Let_Snd: "
     \<lbrakk> 
+      {SND x\<^sub>p} \<subseteq> \<X> x;
       \<forall> x\<^sub>1 x\<^sub>2 . ^Pair x\<^sub>1 x\<^sub>2 \<in> \<V> x\<^sub>p \<longrightarrow> \<V> x\<^sub>2 \<subseteq> \<V> x; 
-      (\<V>, \<C>) \<Turnstile>\<^sub>e e
+      (\<V>, \<C>, \<X>) \<Turnstile>\<^sub>e e
     \<rbrakk> \<Longrightarrow> 
-    (\<V>, \<C>) \<Turnstile>\<^sub>e LET x = SND x\<^sub>p in e
+    (\<V>, \<C>, \<X>) \<Turnstile>\<^sub>e LET x = SND x\<^sub>p in e
   " |
   Let_App: "
     \<lbrakk>
+      {APP f x\<^sub>a} \<subseteq> \<X> x;
       \<forall> f' x' e' . ^Abs f' x' e' \<in> \<V> f \<longrightarrow>
         \<V> x\<^sub>a \<subseteq> \<V> x' \<and>
         \<V> (\<lfloor>e'\<rfloor>) \<subseteq> \<V> x
       ;
-      (\<V>, \<C>) \<Turnstile>\<^sub>e e
+      (\<V>, \<C>, \<X>) \<Turnstile>\<^sub>e e
     \<rbrakk> \<Longrightarrow> 
-    (\<V>, \<C>) \<Turnstile>\<^sub>e LET x = APP f x\<^sub>a in e
+    (\<V>, \<C>, \<X>) \<Turnstile>\<^sub>e LET x = APP f x\<^sub>a in e
   " |
   Let_Sync  : "
     \<lbrakk>
+      {SYNC x\<^sub>e} \<subseteq> \<X> x;
       \<forall> x\<^sub>s\<^sub>c x\<^sub>m x\<^sub>c . 
         ^Send_Evt x\<^sub>s\<^sub>c x\<^sub>m \<in> \<V> x\<^sub>e \<longrightarrow> 
         ^Chan x\<^sub>c \<in> \<V> x\<^sub>s\<^sub>c \<longrightarrow>
@@ -111,24 +127,26 @@ inductive accept_exp :: "abstract_value_env \<times> abstract_value_env \<Righta
         ^Chan x\<^sub>c \<in> \<V> x\<^sub>r\<^sub>c \<longrightarrow>
         \<C> x\<^sub>c \<subseteq> \<V> x
       ;
-      (\<V>, \<C>) \<Turnstile>\<^sub>e e
+      (\<V>, \<C>, \<X>) \<Turnstile>\<^sub>e e
     \<rbrakk> \<Longrightarrow>  
-    (\<V>, \<C>) \<Turnstile>\<^sub>e LET x = SYNC x\<^sub>e in e
+    (\<V>, \<C>, \<X>) \<Turnstile>\<^sub>e LET x = SYNC x\<^sub>e in e
   " |
   Let_Chan: "
     \<lbrakk>
+      {CHAN \<lparr>\<rparr>} \<subseteq> \<X> x;
       {^Chan x} \<subseteq> \<V> x;
-      (\<V>, \<C>) \<Turnstile>\<^sub>e e
+      (\<V>, \<C>, \<X>) \<Turnstile>\<^sub>e e
     \<rbrakk> \<Longrightarrow>  
-    (\<V>, \<C>) \<Turnstile>\<^sub>e LET x = CHAN \<lparr>\<rparr> in e
+    (\<V>, \<C>, \<X>) \<Turnstile>\<^sub>e LET x = CHAN \<lparr>\<rparr> in e
   " |
-  Let_Spawn_Parent: "
+  Let_Spawn: "
     \<lbrakk>
+      {SPAWN e\<^sub>c} \<subseteq> \<X> x;
       {^\<lparr>\<rparr>} \<subseteq> \<V> x;
-      (\<V>, \<C>) \<Turnstile>\<^sub>e e\<^sub>c;
-      (\<V>, \<C>) \<Turnstile>\<^sub>e e
+      (\<V>, \<C>, \<X>) \<Turnstile>\<^sub>e e\<^sub>c;
+      (\<V>, \<C>, \<X>) \<Turnstile>\<^sub>e e
     \<rbrakk> \<Longrightarrow>  
-    (\<V>, \<C>) \<Turnstile>\<^sub>e LET x = SPAWN e\<^sub>c in e
+    (\<V>, \<C>, \<X>) \<Turnstile>\<^sub>e LET x = SPAWN e\<^sub>c in e
   "
 
 
@@ -148,89 +166,89 @@ definition abstract_value_env_precision :: "abstract_value_env \<Rightarrow> abs
   "\<V> \<sqsubseteq> \<V>' \<equiv> (\<forall> x . \<V> x \<subseteq> \<V>' x)"
 
 
-inductive accept_value :: "abstract_value_env \<times> abstract_value_env \<Rightarrow> val \<Rightarrow> bool" (infix "\<Turnstile>\<^sub>\<omega>" 55)
-and  accept_val_env :: "abstract_value_env \<times> abstract_value_env \<Rightarrow> val_env \<Rightarrow> bool" (infix "\<Turnstile>\<^sub>\<rho>" 55) 
+inductive accept_value :: "abstract_value_env \<times> abstract_value_env \<times> bind_env \<Rightarrow> val \<Rightarrow> bool" (infix "\<Turnstile>\<^sub>\<omega>" 55)
+and  accept_val_env :: "abstract_value_env \<times> abstract_value_env \<times> bind_env \<Rightarrow> val_env \<Rightarrow> bool" (infix "\<Turnstile>\<^sub>\<rho>" 55) 
 where
-  Unit: "(\<V>, \<C>) \<Turnstile>\<^sub>\<omega> \<lbrace>\<rbrace>" |
-  Chan: "(\<V>, \<C>) \<Turnstile>\<^sub>\<omega> \<lbrace>c\<rbrace>" |
+  Unit: "(\<V>, \<C>, \<X>) \<Turnstile>\<^sub>\<omega> \<lbrace>\<rbrace>" |
+  Chan: "(\<V>, \<C>, \<X>) \<Turnstile>\<^sub>\<omega> \<lbrace>c\<rbrace>" |
   Abs: "
     \<lbrakk>
       {^Abs f x e} \<subseteq> \<V> f;
-      (\<V>, \<C>) \<Turnstile>\<^sub>e e;
-      (\<V>, \<C>) \<Turnstile>\<^sub>\<rho> \<rho>
+      (\<V>, \<C>, \<X>) \<Turnstile>\<^sub>e e;
+      (\<V>, \<C>, \<X>) \<Turnstile>\<^sub>\<rho> \<rho>
     \<rbrakk> \<Longrightarrow> 
-    (\<V>, \<C>) \<Turnstile>\<^sub>\<omega> \<lbrace>Abs f x e, \<rho>\<rbrace>
+    (\<V>, \<C>, \<X>) \<Turnstile>\<^sub>\<omega> \<lbrace>Abs f x e, \<rho>\<rbrace>
   " |
   Pair: "
-    (\<V>, \<C>) \<Turnstile>\<^sub>\<rho> \<rho>
+    (\<V>, \<C>, \<X>) \<Turnstile>\<^sub>\<rho> \<rho>
     \<Longrightarrow>
-    (\<V>, \<C>) \<Turnstile>\<^sub>\<omega> \<lbrace>Pair _ _, \<rho>\<rbrace>
+    (\<V>, \<C>, \<X>) \<Turnstile>\<^sub>\<omega> \<lbrace>Pair _ _, \<rho>\<rbrace>
   " |
   Left: "
-    (\<V>, \<C>) \<Turnstile>\<^sub>\<rho> \<rho>
+    (\<V>, \<C>, \<X>) \<Turnstile>\<^sub>\<rho> \<rho>
     \<Longrightarrow>
-    (\<V>, \<C>) \<Turnstile>\<^sub>\<omega> \<lbrace>Left _, \<rho>\<rbrace>
+    (\<V>, \<C>, \<X>) \<Turnstile>\<^sub>\<omega> \<lbrace>Left _, \<rho>\<rbrace>
   " |
   Right: "
-    (\<V>, \<C>) \<Turnstile>\<^sub>\<rho> \<rho>
+    (\<V>, \<C>, \<X>) \<Turnstile>\<^sub>\<rho> \<rho>
     \<Longrightarrow>
-    (\<V>, \<C>) \<Turnstile>\<^sub>\<omega> \<lbrace>Right _, \<rho>\<rbrace>
+    (\<V>, \<C>, \<X>) \<Turnstile>\<^sub>\<omega> \<lbrace>Right _, \<rho>\<rbrace>
   " |
   Send_Evt: "
-    (\<V>, \<C>) \<Turnstile>\<^sub>\<rho> \<rho>
+    (\<V>, \<C>, \<X>) \<Turnstile>\<^sub>\<rho> \<rho>
     \<Longrightarrow>
-    (\<V>, \<C>) \<Turnstile>\<^sub>\<omega> \<lbrace>Send_Evt _ _, \<rho>\<rbrace>
+    (\<V>, \<C>, \<X>) \<Turnstile>\<^sub>\<omega> \<lbrace>Send_Evt _ _, \<rho>\<rbrace>
   " |
   Recv_Evt: "
-    (\<V>, \<C>) \<Turnstile>\<^sub>\<rho> \<rho>
+    (\<V>, \<C>, \<X>) \<Turnstile>\<^sub>\<rho> \<rho>
     \<Longrightarrow>
-    (\<V>, \<C>) \<Turnstile>\<^sub>\<omega> \<lbrace>Recv_Evt _, \<rho>\<rbrace>
+    (\<V>, \<C>, \<X>) \<Turnstile>\<^sub>\<omega> \<lbrace>Recv_Evt _, \<rho>\<rbrace>
   " |
   Always_Evt: "
-    (\<V>, \<C>) \<Turnstile>\<^sub>\<rho> \<rho>
+    (\<V>, \<C>, \<X>) \<Turnstile>\<^sub>\<rho> \<rho>
     \<Longrightarrow>
-    (\<V>, \<C>) \<Turnstile>\<^sub>\<omega> \<lbrace>Always_Evt _, \<rho>\<rbrace>
+    (\<V>, \<C>, \<X>) \<Turnstile>\<^sub>\<omega> \<lbrace>Always_Evt _, \<rho>\<rbrace>
   " |
 
   Any : "
     \<lbrakk>
       (\<forall> x \<omega> . \<rho> x = Some \<omega> \<longrightarrow>
-        {|\<omega>|} \<subseteq> \<V> x \<and> (\<V>, \<C>) \<Turnstile>\<^sub>\<omega> \<omega>
+        {|\<omega>|} \<subseteq> \<V> x \<and> (\<V>, \<C>, \<X>) \<Turnstile>\<^sub>\<omega> \<omega>
       )
     \<rbrakk> \<Longrightarrow>
-    (\<V>, \<C>) \<Turnstile>\<^sub>\<rho> \<rho>
+    (\<V>, \<C>, \<X>) \<Turnstile>\<^sub>\<rho> \<rho>
   "
 
 
-inductive accept_stack :: "abstract_value_env \<times> abstract_value_env \<Rightarrow> abstract_value set \<Rightarrow> cont list \<Rightarrow> bool" ("_ \<Turnstile>\<^sub>\<kappa> _ \<Rrightarrow> _" [56,0,56]55) where
-  Empty: "(\<V>, \<C>) \<Turnstile>\<^sub>\<kappa> \<W> \<Rrightarrow> []" |
+inductive accept_stack :: "abstract_value_env \<times> abstract_value_env \<times> bind_env \<Rightarrow> abstract_value set \<Rightarrow> cont list \<Rightarrow> bool" ("_ \<Turnstile>\<^sub>\<kappa> _ \<Rrightarrow> _" [56,0,56]55) where
+  Empty: "(\<V>, \<C>, \<X>) \<Turnstile>\<^sub>\<kappa> \<W> \<Rrightarrow> []" |
   Nonempty: "
     \<lbrakk> 
       \<W> \<subseteq> \<V> x;
-      (\<V>, \<C>) \<Turnstile>\<^sub>e e;
-      (\<V>, \<C>) \<Turnstile>\<^sub>\<rho> \<rho>; 
-      (\<V>, \<C>) \<Turnstile>\<^sub>\<kappa> \<V> (\<lfloor>e\<rfloor>) \<Rrightarrow> \<kappa>
+      (\<V>, \<C>, \<X>) \<Turnstile>\<^sub>e e;
+      (\<V>, \<C>, \<X>) \<Turnstile>\<^sub>\<rho> \<rho>; 
+      (\<V>, \<C>, \<X>) \<Turnstile>\<^sub>\<kappa> \<V> (\<lfloor>e\<rfloor>) \<Rrightarrow> \<kappa>
     \<rbrakk> \<Longrightarrow> 
-    (\<V>, \<C>) \<Turnstile>\<^sub>\<kappa> \<W> \<Rrightarrow> (\<langle>x, e, \<rho>\<rangle> # \<kappa>)
+    (\<V>, \<C>, \<X>) \<Turnstile>\<^sub>\<kappa> \<W> \<Rrightarrow> (\<langle>x, e, \<rho>\<rangle> # \<kappa>)
   "
 
 
-inductive accept_state :: "abstract_value_env \<times> abstract_value_env \<Rightarrow> state \<Rightarrow> bool" (infix "\<Turnstile>\<^sub>\<sigma>" 55)  where
+inductive accept_state :: "abstract_value_env \<times> abstract_value_env \<times> bind_env \<Rightarrow> state \<Rightarrow> bool" (infix "\<Turnstile>\<^sub>\<sigma>" 55)  where
   Any: "
     \<lbrakk>
-      (\<V>, \<C>) \<Turnstile>\<^sub>e e; 
-      (\<V>, \<C>) \<Turnstile>\<^sub>\<rho> \<rho>; 
-      (\<V>, \<C>) \<Turnstile>\<^sub>\<kappa> \<V> (\<lfloor>e\<rfloor>) \<Rrightarrow> \<kappa>
+      (\<V>, \<C>, \<X>) \<Turnstile>\<^sub>e e; 
+      (\<V>, \<C>, \<X>) \<Turnstile>\<^sub>\<rho> \<rho>; 
+      (\<V>, \<C>, \<X>) \<Turnstile>\<^sub>\<kappa> \<V> (\<lfloor>e\<rfloor>) \<Rrightarrow> \<kappa>
     \<rbrakk> \<Longrightarrow>
-    (\<V>, \<C>) \<Turnstile>\<^sub>\<sigma> \<langle>e; \<rho>; \<kappa>\<rangle>
+    (\<V>, \<C>, \<X>) \<Turnstile>\<^sub>\<sigma> \<langle>e; \<rho>; \<kappa>\<rangle>
   "
 
 
-inductive accept_state_pool :: "abstract_value_env \<times> abstract_value_env \<Rightarrow> state_pool \<Rightarrow> bool" (infix "\<Turnstile>\<^sub>\<E>" 55) where
+inductive accept_state_pool :: "abstract_value_env \<times> abstract_value_env \<times> bind_env \<Rightarrow> state_pool \<Rightarrow> bool" (infix "\<Turnstile>\<^sub>\<E>" 55) where
   Any: "
-    (\<forall> \<pi> \<sigma> . \<E> \<pi> = Some \<sigma> \<longrightarrow> (\<V>, \<C>) \<Turnstile>\<^sub>\<sigma> \<sigma>)
+    (\<forall> \<pi> \<sigma> . \<E> \<pi> = Some \<sigma> \<longrightarrow> (\<V>, \<C>, \<X>) \<Turnstile>\<^sub>\<sigma> \<sigma>)
     \<Longrightarrow> 
-    (\<V>, \<C>) \<Turnstile>\<^sub>\<E> \<E>
+    (\<V>, \<C>, \<X>) \<Turnstile>\<^sub>\<E> \<E>
   "
    
 end
