Abstract_Value_Flow_Soundness.thy
@@ -4,15 +4,15 @@ begin
 
 
 lemma flow_state_to_flow_exp: "
-  (\<V>, \<C>) \<Turnstile>\<^sub>\<sigma> \<langle>RESULT x;\<rho>;\<langle>x\<^sub>\<kappa>,e\<^sub>\<kappa>,\<rho>\<^sub>\<kappa>\<rangle> # \<kappa>\<rangle> \<Longrightarrow> \<rho> x = Some \<omega> \<Longrightarrow> (\<V>, \<C>) \<Turnstile>\<^sub>e  e\<^sub>\<kappa>
+  (\<V>, \<C>, \<X>) \<Turnstile>\<^sub>\<sigma> \<langle>RESULT x;\<rho>;\<langle>x\<^sub>\<kappa>,e\<^sub>\<kappa>,\<rho>\<^sub>\<kappa>\<rangle> # \<kappa>\<rangle> \<Longrightarrow> \<rho> x = Some \<omega> \<Longrightarrow> (\<V>, \<C>, \<X>) \<Turnstile>\<^sub>e  e\<^sub>\<kappa>
 "
  apply (erule accept_state.cases, auto)
  apply (erule accept_stack.cases, auto)
 done
 
 lemma flow_over_state_to_env: "
-  (\<V>, \<C>) \<Turnstile>\<^sub>\<sigma>  \<langle>RESULT x; \<rho>; \<langle>x\<^sub>\<kappa>,e\<^sub>\<kappa>,\<rho>\<^sub>\<kappa>\<rangle> # \<kappa>\<rangle> \<Longrightarrow> \<rho> x = Some \<omega> \<Longrightarrow> 
-  (\<V>, \<C>) \<Turnstile>\<^sub>\<rho> \<rho>\<^sub>\<kappa>(x\<^sub>\<kappa> \<mapsto> \<omega>)
+  (\<V>, \<C>, \<X>) \<Turnstile>\<^sub>\<sigma>  \<langle>RESULT x; \<rho>; \<langle>x\<^sub>\<kappa>,e\<^sub>\<kappa>,\<rho>\<^sub>\<kappa>\<rangle> # \<kappa>\<rangle> \<Longrightarrow> \<rho> x = Some \<omega> \<Longrightarrow> 
+  (\<V>, \<C>, \<X>) \<Turnstile>\<^sub>\<rho> \<rho>\<^sub>\<kappa>(x\<^sub>\<kappa> \<mapsto> \<omega>)
 "
  apply (rule accept_value_accept_val_env.Any, auto)
       apply (erule accept_state.cases, auto)
@@ -35,7 +35,7 @@ lemma flow_over_state_to_env: "
 done
 
 lemma flow_over_state_to_stack: "
-  (\<V>, \<C>) \<Turnstile>\<^sub>\<sigma>  \<langle>RESULT x; \<rho>; \<langle>x\<^sub>\<kappa>,e\<^sub>\<kappa>,\<rho>\<^sub>\<kappa>\<rangle> # \<kappa>\<rangle> \<Longrightarrow> \<rho> x = Some \<omega> \<Longrightarrow> (\<V>, \<C>) \<Turnstile>\<^sub>\<kappa>  \<V> (\<lfloor>e\<^sub>\<kappa>\<rfloor>) \<Rrightarrow> \<kappa>
+  (\<V>, \<C>, \<X>) \<Turnstile>\<^sub>\<sigma>  \<langle>RESULT x; \<rho>; \<langle>x\<^sub>\<kappa>,e\<^sub>\<kappa>,\<rho>\<^sub>\<kappa>\<rangle> # \<kappa>\<rangle> \<Longrightarrow> \<rho> x = Some \<omega> \<Longrightarrow> (\<V>, \<C>, \<X>) \<Turnstile>\<^sub>\<kappa>  \<V> (\<lfloor>e\<^sub>\<kappa>\<rfloor>) \<Rrightarrow> \<kappa>
 "
  apply (erule accept_state.cases, auto)
  apply (erule accept_val_env.cases, auto)
@@ -45,7 +45,7 @@ lemma flow_over_state_to_stack: "
 done
 
 lemma flow_over_state_1: "
-  (\<V>, \<C>) \<Turnstile>\<^sub>\<sigma>  \<langle>RESULT x; \<rho>; \<langle>x\<^sub>\<kappa>,e\<^sub>\<kappa>,\<rho>\<^sub>\<kappa>\<rangle> # \<kappa>\<rangle> \<Longrightarrow> \<rho> x = Some \<omega> \<Longrightarrow> (\<V>, \<C>) \<Turnstile>\<^sub>\<sigma>  \<langle>e\<^sub>\<kappa>; \<rho>\<^sub>\<kappa>(x\<^sub>\<kappa> \<mapsto> \<omega>); \<kappa>\<rangle>
+  (\<V>, \<C>, \<X>) \<Turnstile>\<^sub>\<sigma>  \<langle>RESULT x; \<rho>; \<langle>x\<^sub>\<kappa>,e\<^sub>\<kappa>,\<rho>\<^sub>\<kappa>\<rangle> # \<kappa>\<rangle> \<Longrightarrow> \<rho> x = Some \<omega> \<Longrightarrow> (\<V>, \<C>, \<X>) \<Turnstile>\<^sub>\<sigma>  \<langle>e\<^sub>\<kappa>; \<rho>\<^sub>\<kappa>(x\<^sub>\<kappa> \<mapsto> \<omega>); \<kappa>\<rangle>
 "
  apply (rule accept_state.Any)
     apply (erule flow_state_to_flow_exp, auto)
@@ -54,14 +54,14 @@ lemma flow_over_state_1: "
 done
 
 lemma flow_state_to_flow_exp_2: "
-  (\<V>, \<C>) \<Turnstile>\<^sub>\<sigma>  \<langle>LET x = \<lparr>\<rparr> in e; \<rho>; \<kappa>\<rangle> \<Longrightarrow> (\<V>, \<C>) \<Turnstile>\<^sub>e  e
+  (\<V>, \<C>, \<X>) \<Turnstile>\<^sub>\<sigma>  \<langle>LET x = \<lparr>\<rparr> in e; \<rho>; \<kappa>\<rangle> \<Longrightarrow> (\<V>, \<C>, \<X>) \<Turnstile>\<^sub>e  e
 "
  apply (erule accept_state.cases, auto)
  apply (erule accept_exp.cases, auto)
 done
 
 lemma flow_over_state_to_env_2: "
-  (\<V>, \<C>) \<Turnstile>\<^sub>\<sigma>  \<langle>LET x = \<lparr>\<rparr> in e; \<rho>; \<kappa>\<rangle> \<Longrightarrow> (\<V>, \<C>) \<Turnstile>\<^sub>\<rho> \<rho>(x \<mapsto> \<lbrace>\<rbrace>)
+  (\<V>, \<C>, \<X>) \<Turnstile>\<^sub>\<sigma>  \<langle>LET x = \<lparr>\<rparr> in e; \<rho>; \<kappa>\<rangle> \<Longrightarrow> (\<V>, \<C>, \<X>) \<Turnstile>\<^sub>\<rho> \<rho>(x \<mapsto> \<lbrace>\<rbrace>)
 "
  apply (rule accept_value_accept_val_env.Any, auto)
      apply (erule accept_state.cases, auto)
@@ -75,13 +75,13 @@ lemma flow_over_state_to_env_2: "
 done
 
 lemma flow_over_state_to_stack_2: "
-  (\<V>, \<C>) \<Turnstile>\<^sub>\<sigma>  \<langle>LET x = \<lparr>\<rparr> in e; \<rho>; \<kappa>\<rangle> \<Longrightarrow> (\<V>, \<C>) \<Turnstile>\<^sub>\<kappa>  \<V> (\<lfloor>e\<rfloor>) \<Rrightarrow> \<kappa>
+  (\<V>, \<C>, \<X>) \<Turnstile>\<^sub>\<sigma>  \<langle>LET x = \<lparr>\<rparr> in e; \<rho>; \<kappa>\<rangle> \<Longrightarrow> (\<V>, \<C>, \<X>) \<Turnstile>\<^sub>\<kappa>  \<V> (\<lfloor>e\<rfloor>) \<Rrightarrow> \<kappa>
 "
  apply (erule accept_state.cases, auto)
 done
 
 lemma flow_over_state_2: "
-  (\<V>, \<C>) \<Turnstile>\<^sub>\<sigma>  \<langle>LET x = \<lparr>\<rparr> in e; \<rho>; \<kappa>\<rangle> \<Longrightarrow> (\<V>, \<C>) \<Turnstile>\<^sub>\<sigma>  \<langle>e; \<rho>(x \<mapsto> \<lbrace>\<rbrace>); \<kappa>\<rangle>
+  (\<V>, \<C>, \<X>) \<Turnstile>\<^sub>\<sigma>  \<langle>LET x = \<lparr>\<rparr> in e; \<rho>; \<kappa>\<rangle> \<Longrightarrow> (\<V>, \<C>, \<X>) \<Turnstile>\<^sub>\<sigma>  \<langle>e; \<rho>(x \<mapsto> \<lbrace>\<rbrace>); \<kappa>\<rangle>
 "
  apply (rule accept_state.Any)
     apply (erule flow_state_to_flow_exp_2)
@@ -90,14 +90,14 @@ lemma flow_over_state_2: "
 done
 
 lemma flow_over_state_to_exp_3: "
-  (\<V>, \<C>) \<Turnstile>\<^sub>\<sigma>  \<langle>LET x = Prim p in e; \<rho>; \<kappa>\<rangle> \<Longrightarrow> (\<V>, \<C>) \<Turnstile>\<^sub>e  e
+  (\<V>, \<C>, \<X>) \<Turnstile>\<^sub>\<sigma>  \<langle>LET x = Prim p in e; \<rho>; \<kappa>\<rangle> \<Longrightarrow> (\<V>, \<C>, \<X>) \<Turnstile>\<^sub>e  e
 "
  apply (erule accept_state.cases, auto)  
  apply (erule accept_exp.cases, auto)
 done
 
 lemma flow_over_state_to_env_3: "
-  (\<V>, \<C>) \<Turnstile>\<^sub>\<sigma>  \<langle>LET x = Prim p in e; \<rho>; \<kappa>\<rangle> \<Longrightarrow> (\<V>, \<C>) \<Turnstile>\<^sub>\<rho> \<rho>(x \<mapsto> \<lbrace>p, \<rho>\<rbrace>)
+  (\<V>, \<C>, \<X>) \<Turnstile>\<^sub>\<sigma>  \<langle>LET x = Prim p in e; \<rho>; \<kappa>\<rangle> \<Longrightarrow> (\<V>, \<C>, \<X>) \<Turnstile>\<^sub>\<rho> \<rho>(x \<mapsto> \<lbrace>p, \<rho>\<rbrace>)
 "
  apply (rule accept_value_accept_val_env.Any, auto)
      apply (erule accept_state.cases, auto)
@@ -112,13 +112,13 @@ lemma flow_over_state_to_env_3: "
 done
 
 lemma flow_over_state_to_stack_3: "
-  (\<V>, \<C>) \<Turnstile>\<^sub>\<sigma>  \<langle>LET x = Prim p in e; \<rho>; \<kappa>\<rangle> \<Longrightarrow> (\<V>, \<C>) \<Turnstile>\<^sub>\<kappa>  \<V> (\<lfloor>e\<rfloor>) \<Rrightarrow> \<kappa>
+  (\<V>, \<C>, \<X>) \<Turnstile>\<^sub>\<sigma>  \<langle>LET x = Prim p in e; \<rho>; \<kappa>\<rangle> \<Longrightarrow> (\<V>, \<C>, \<X>) \<Turnstile>\<^sub>\<kappa>  \<V> (\<lfloor>e\<rfloor>) \<Rrightarrow> \<kappa>
 "
  apply (erule accept_state.cases, auto)
 done
 
 lemma flow_over_state_3: "
-  (\<V>, \<C>) \<Turnstile>\<^sub>\<sigma>  \<langle>LET x = Prim p in e; \<rho>; \<kappa>\<rangle> \<Longrightarrow>  (\<V>, \<C>) \<Turnstile>\<^sub>\<sigma>  \<langle>e; \<rho>(x \<mapsto> \<lbrace>p, \<rho>\<rbrace>); \<kappa>\<rangle>
+  (\<V>, \<C>, \<X>) \<Turnstile>\<^sub>\<sigma>  \<langle>LET x = Prim p in e; \<rho>; \<kappa>\<rangle> \<Longrightarrow>  (\<V>, \<C>, \<X>) \<Turnstile>\<^sub>\<sigma>  \<langle>e; \<rho>(x \<mapsto> \<lbrace>p, \<rho>\<rbrace>); \<kappa>\<rangle>
 "
  apply (rule accept_state.Any)
     apply (erule flow_over_state_to_exp_3)
@@ -127,9 +127,9 @@ lemma flow_over_state_3: "
 done
 
 lemma flow_state_to_flow_exp_4: "
-  (\<V>, \<C>) \<Turnstile>\<^sub>\<sigma>  \<langle>LET x = CASE x\<^sub>s LEFT x\<^sub>l |> e\<^sub>l RIGHT x\<^sub>r |> e\<^sub>r in e; \<rho>; \<kappa>\<rangle> \<Longrightarrow> 
+  (\<V>, \<C>, \<X>) \<Turnstile>\<^sub>\<sigma>  \<langle>LET x = CASE x\<^sub>s LEFT x\<^sub>l |> e\<^sub>l RIGHT x\<^sub>r |> e\<^sub>r in e; \<rho>; \<kappa>\<rangle> \<Longrightarrow> 
   \<rho> x\<^sub>s = Some \<lbrace>prim.Left x\<^sub>l', \<rho>\<^sub>l\<rbrace> \<Longrightarrow> 
-  \<rho>\<^sub>l x\<^sub>l' = Some \<omega>\<^sub>l \<Longrightarrow> (\<V>, \<C>) \<Turnstile>\<^sub>e  e\<^sub>l
+  \<rho>\<^sub>l x\<^sub>l' = Some \<omega>\<^sub>l \<Longrightarrow> (\<V>, \<C>, \<X>) \<Turnstile>\<^sub>e  e\<^sub>l
 "
  apply (erule accept_state.cases, auto)
  apply (erule accept_exp.cases, auto)
@@ -138,9 +138,9 @@ lemma flow_state_to_flow_exp_4: "
 done
 
 lemma flow_state_to_flow_env_4: "
-  (\<V>, \<C>) \<Turnstile>\<^sub>\<sigma>  \<langle>LET x = CASE x\<^sub>s LEFT x\<^sub>l |> e\<^sub>l RIGHT x\<^sub>r |> e\<^sub>r in e; \<rho>; \<kappa>\<rangle> \<Longrightarrow> 
+  (\<V>, \<C>, \<X>) \<Turnstile>\<^sub>\<sigma>  \<langle>LET x = CASE x\<^sub>s LEFT x\<^sub>l |> e\<^sub>l RIGHT x\<^sub>r |> e\<^sub>r in e; \<rho>; \<kappa>\<rangle> \<Longrightarrow> 
   \<rho> x\<^sub>s = Some \<lbrace>prim.Left x\<^sub>l', \<rho>\<^sub>l\<rbrace> \<Longrightarrow> \<rho>\<^sub>l x\<^sub>l' = Some \<omega>\<^sub>l \<Longrightarrow> 
-  (\<V>, \<C>) \<Turnstile>\<^sub>\<rho> \<rho>(x\<^sub>l \<mapsto> \<omega>\<^sub>l)
+  (\<V>, \<C>, \<X>) \<Turnstile>\<^sub>\<rho> \<rho>(x\<^sub>l \<mapsto> \<omega>\<^sub>l)
 "
  apply (rule accept_value_accept_val_env.Any, auto)
       apply (erule accept_state.cases, auto)
@@ -164,9 +164,9 @@ lemma flow_state_to_flow_env_4: "
 done
 
 lemma flow_state_to_flow_stack_4: "
-  (\<V>, \<C>) \<Turnstile>\<^sub>\<sigma>  \<langle>LET x = CASE x\<^sub>s LEFT x\<^sub>l |> e\<^sub>l RIGHT x\<^sub>r |> e\<^sub>r in e; \<rho>; \<kappa>\<rangle> \<Longrightarrow>
+  (\<V>, \<C>, \<X>) \<Turnstile>\<^sub>\<sigma>  \<langle>LET x = CASE x\<^sub>s LEFT x\<^sub>l |> e\<^sub>l RIGHT x\<^sub>r |> e\<^sub>r in e; \<rho>; \<kappa>\<rangle> \<Longrightarrow>
   \<rho> x\<^sub>s = Some \<lbrace>prim.Left x\<^sub>l', \<rho>\<^sub>l\<rbrace> \<Longrightarrow> \<rho>\<^sub>l x\<^sub>l' = Some \<omega>\<^sub>l \<Longrightarrow> 
-  (\<V>, \<C>) \<Turnstile>\<^sub>\<kappa> \<V> (\<lfloor>e\<^sub>l\<rfloor>) \<Rrightarrow> \<langle>x,e,\<rho>\<rangle> # \<kappa>
+  (\<V>, \<C>, \<X>) \<Turnstile>\<^sub>\<kappa> \<V> (\<lfloor>e\<^sub>l\<rfloor>) \<Rrightarrow> \<langle>x,e,\<rho>\<rangle> # \<kappa>
 "
  apply (rule accept_stack.Nonempty)
     apply (erule accept_state.cases, auto, rename_tac \<omega>)
@@ -180,9 +180,9 @@ lemma flow_state_to_flow_stack_4: "
 done
 
 lemma flow_over_state_4: "
-  (\<V>, \<C>) \<Turnstile>\<^sub>\<sigma>  \<langle>LET x = CASE x\<^sub>s LEFT x\<^sub>l |> e\<^sub>l RIGHT x\<^sub>r |> e\<^sub>r in e; \<rho>; \<kappa>\<rangle> \<Longrightarrow> 
+  (\<V>, \<C>, \<X>) \<Turnstile>\<^sub>\<sigma>  \<langle>LET x = CASE x\<^sub>s LEFT x\<^sub>l |> e\<^sub>l RIGHT x\<^sub>r |> e\<^sub>r in e; \<rho>; \<kappa>\<rangle> \<Longrightarrow> 
   \<rho> x\<^sub>s = Some \<lbrace>prim.Left x\<^sub>l', \<rho>\<^sub>l\<rbrace> \<Longrightarrow> 
-  \<rho>\<^sub>l x\<^sub>l' = Some \<omega>\<^sub>l \<Longrightarrow> (\<V>, \<C>) \<Turnstile>\<^sub>\<sigma>  \<langle>e\<^sub>l; \<rho>(x\<^sub>l \<mapsto> \<omega>\<^sub>l); \<langle>x,e,\<rho>\<rangle> # \<kappa>\<rangle>
+  \<rho>\<^sub>l x\<^sub>l' = Some \<omega>\<^sub>l \<Longrightarrow> (\<V>, \<C>, \<X>) \<Turnstile>\<^sub>\<sigma>  \<langle>e\<^sub>l; \<rho>(x\<^sub>l \<mapsto> \<omega>\<^sub>l); \<langle>x,e,\<rho>\<rangle> # \<kappa>\<rangle>
 "
  apply (rule accept_state.Any)
     apply (erule flow_state_to_flow_exp_4, simp, auto)
@@ -191,9 +191,9 @@ lemma flow_over_state_4: "
 done
 
 lemma flow_state_to_flow_exp_5: "
-  (\<V>, \<C>) \<Turnstile>\<^sub>\<sigma>  \<langle>LET x = CASE x\<^sub>s LEFT x\<^sub>l |> e\<^sub>l RIGHT x\<^sub>r |> e\<^sub>r in e; \<rho>; \<kappa>\<rangle> \<Longrightarrow> 
+  (\<V>, \<C>, \<X>) \<Turnstile>\<^sub>\<sigma>  \<langle>LET x = CASE x\<^sub>s LEFT x\<^sub>l |> e\<^sub>l RIGHT x\<^sub>r |> e\<^sub>r in e; \<rho>; \<kappa>\<rangle> \<Longrightarrow> 
   \<rho> x\<^sub>s = Some \<lbrace>prim.Right x\<^sub>r', \<rho>\<^sub>r\<rbrace> \<Longrightarrow> 
-  \<rho>\<^sub>r x\<^sub>r' = Some \<omega>\<^sub>r \<Longrightarrow> (\<V>, \<C>) \<Turnstile>\<^sub>e  e\<^sub>r
+  \<rho>\<^sub>r x\<^sub>r' = Some \<omega>\<^sub>r \<Longrightarrow> (\<V>, \<C>, \<X>) \<Turnstile>\<^sub>e  e\<^sub>r
 "
  apply (erule accept_state.cases, auto)
  apply (erule accept_exp.cases, auto)
@@ -202,9 +202,9 @@ lemma flow_state_to_flow_exp_5: "
 done
 
 lemma flow_state_to_flow_env_5: "
-  (\<V>, \<C>) \<Turnstile>\<^sub>\<sigma>  \<langle>LET x = CASE x\<^sub>s LEFT x\<^sub>l |> e\<^sub>l RIGHT x\<^sub>r |> e\<^sub>r in e; \<rho>; \<kappa>\<rangle> \<Longrightarrow> 
+  (\<V>, \<C>, \<X>) \<Turnstile>\<^sub>\<sigma>  \<langle>LET x = CASE x\<^sub>s LEFT x\<^sub>l |> e\<^sub>l RIGHT x\<^sub>r |> e\<^sub>r in e; \<rho>; \<kappa>\<rangle> \<Longrightarrow> 
   \<rho> x\<^sub>s = Some \<lbrace>prim.Right x\<^sub>r', \<rho>\<^sub>r\<rbrace> \<Longrightarrow> \<rho>\<^sub>r x\<^sub>r' = Some \<omega>\<^sub>r \<Longrightarrow> 
-  (\<V>, \<C>) \<Turnstile>\<^sub>\<rho> \<rho>(x\<^sub>r \<mapsto> \<omega>\<^sub>r)
+  (\<V>, \<C>, \<X>) \<Turnstile>\<^sub>\<rho> \<rho>(x\<^sub>r \<mapsto> \<omega>\<^sub>r)
 "
  apply (rule accept_value_accept_val_env.Any, auto)
       apply (erule accept_state.cases, auto)
@@ -228,9 +228,9 @@ lemma flow_state_to_flow_env_5: "
 done
 
 lemma flow_state_to_flow_stack_5: "
-  (\<V>, \<C>) \<Turnstile>\<^sub>\<sigma>  \<langle>LET x = CASE x\<^sub>s LEFT x\<^sub>l |> e\<^sub>l RIGHT x\<^sub>r |> e\<^sub>r in e; \<rho>; \<kappa>\<rangle> \<Longrightarrow>
+  (\<V>, \<C>, \<X>) \<Turnstile>\<^sub>\<sigma>  \<langle>LET x = CASE x\<^sub>s LEFT x\<^sub>l |> e\<^sub>l RIGHT x\<^sub>r |> e\<^sub>r in e; \<rho>; \<kappa>\<rangle> \<Longrightarrow>
   \<rho> x\<^sub>s = Some \<lbrace>prim.Right x\<^sub>r', \<rho>\<^sub>r\<rbrace> \<Longrightarrow> \<rho>\<^sub>r x\<^sub>r' = Some \<omega>\<^sub>r \<Longrightarrow> 
-  (\<V>, \<C>) \<Turnstile>\<^sub>\<kappa>  \<V> (\<lfloor>e\<^sub>r\<rfloor>) \<Rrightarrow> \<langle>x,e,\<rho>\<rangle> # \<kappa>
+  (\<V>, \<C>, \<X>) \<Turnstile>\<^sub>\<kappa>  \<V> (\<lfloor>e\<^sub>r\<rfloor>) \<Rrightarrow> \<langle>x,e,\<rho>\<rangle> # \<kappa>
 "
  apply (rule accept_stack.Nonempty)
     apply (erule accept_state.cases, auto, rename_tac \<omega>)
@@ -244,9 +244,9 @@ lemma flow_state_to_flow_stack_5: "
 done
 
 lemma flow_over_state_5: "
-  (\<V>, \<C>) \<Turnstile>\<^sub>\<sigma>  \<langle>LET x = CASE x\<^sub>s LEFT x\<^sub>l |> e\<^sub>l RIGHT x\<^sub>r |> e\<^sub>r in e; \<rho>; \<kappa>\<rangle> \<Longrightarrow> 
+  (\<V>, \<C>, \<X>) \<Turnstile>\<^sub>\<sigma>  \<langle>LET x = CASE x\<^sub>s LEFT x\<^sub>l |> e\<^sub>l RIGHT x\<^sub>r |> e\<^sub>r in e; \<rho>; \<kappa>\<rangle> \<Longrightarrow> 
   \<rho> x\<^sub>s = Some \<lbrace>prim.Right x\<^sub>r', \<rho>\<^sub>r\<rbrace> \<Longrightarrow> 
-  \<rho>\<^sub>r x\<^sub>r' = Some \<omega>\<^sub>r \<Longrightarrow> (\<V>, \<C>) \<Turnstile>\<^sub>\<sigma>  \<langle>e\<^sub>r; \<rho>(x\<^sub>r \<mapsto> \<omega>\<^sub>r); \<langle>x,e,\<rho>\<rangle> # \<kappa>\<rangle>
+  \<rho>\<^sub>r x\<^sub>r' = Some \<omega>\<^sub>r \<Longrightarrow> (\<V>, \<C>, \<X>) \<Turnstile>\<^sub>\<sigma>  \<langle>e\<^sub>r; \<rho>(x\<^sub>r \<mapsto> \<omega>\<^sub>r); \<langle>x,e,\<rho>\<rangle> # \<kappa>\<rangle>
 "
  apply (rule accept_state.Any)
     apply (erule flow_state_to_flow_exp_5, simp, auto)
@@ -256,15 +256,15 @@ done
 
 
 lemma flow_state_to_flow_exp_6: "
-  (\<V>, \<C>) \<Turnstile>\<^sub>\<sigma>  \<langle>LET x = FST x\<^sub>p in e; \<rho>; \<kappa>\<rangle> \<Longrightarrow> \<rho> x\<^sub>p = Some \<lbrace>prim.Pair x\<^sub>1 x\<^sub>2, \<rho>\<^sub>p\<rbrace> \<Longrightarrow> 
-  \<rho>\<^sub>p x\<^sub>1 = Some \<omega> \<Longrightarrow> (\<V>, \<C>) \<Turnstile>\<^sub>e  e
+  (\<V>, \<C>, \<X>) \<Turnstile>\<^sub>\<sigma>  \<langle>LET x = FST x\<^sub>p in e; \<rho>; \<kappa>\<rangle> \<Longrightarrow> \<rho> x\<^sub>p = Some \<lbrace>prim.Pair x\<^sub>1 x\<^sub>2, \<rho>\<^sub>p\<rbrace> \<Longrightarrow> 
+  \<rho>\<^sub>p x\<^sub>1 = Some \<omega> \<Longrightarrow> (\<V>, \<C>, \<X>) \<Turnstile>\<^sub>e  e
 "
  apply (erule accept_state.cases, auto)
  apply (erule accept_exp.cases, auto)
 done
 
 lemma flow_state_to_flow_env_6: "
-  (\<V>, \<C>) \<Turnstile>\<^sub>\<sigma>  \<langle>LET x = FST x\<^sub>p in e; \<rho>; \<kappa>\<rangle> \<Longrightarrow> \<rho> x\<^sub>p = Some \<lbrace>prim.Pair x\<^sub>1 x\<^sub>2, \<rho>\<^sub>p\<rbrace> \<Longrightarrow> \<rho>\<^sub>p x\<^sub>1 = Some \<omega> \<Longrightarrow> (\<V>, \<C>) \<Turnstile>\<^sub>\<rho> \<rho>(x \<mapsto> \<omega>)
+  (\<V>, \<C>, \<X>) \<Turnstile>\<^sub>\<sigma>  \<langle>LET x = FST x\<^sub>p in e; \<rho>; \<kappa>\<rangle> \<Longrightarrow> \<rho> x\<^sub>p = Some \<lbrace>prim.Pair x\<^sub>1 x\<^sub>2, \<rho>\<^sub>p\<rbrace> \<Longrightarrow> \<rho>\<^sub>p x\<^sub>1 = Some \<omega> \<Longrightarrow> (\<V>, \<C>, \<X>) \<Turnstile>\<^sub>\<rho> \<rho>(x \<mapsto> \<omega>)
 "
  apply (rule accept_value_accept_val_env.Any, auto)
       apply (erule accept_state.cases, auto)
@@ -288,15 +288,15 @@ lemma flow_state_to_flow_env_6: "
 done
 
 lemma flow_state_to_flow_stack_6: "
-  (\<V>, \<C>) \<Turnstile>\<^sub>\<sigma>  \<langle>LET x = FST x\<^sub>p in e; \<rho>; \<kappa>\<rangle> \<Longrightarrow> \<rho> x\<^sub>p = Some \<lbrace>prim.Pair x\<^sub>1 x\<^sub>2, \<rho>\<^sub>p\<rbrace> \<Longrightarrow> \<rho>\<^sub>p x\<^sub>1 = Some \<omega> \<Longrightarrow> (\<V>, \<C>) \<Turnstile>\<^sub>\<kappa>  \<V> (\<lfloor>e\<rfloor>) \<Rrightarrow> \<kappa>
+  (\<V>, \<C>, \<X>) \<Turnstile>\<^sub>\<sigma>  \<langle>LET x = FST x\<^sub>p in e; \<rho>; \<kappa>\<rangle> \<Longrightarrow> \<rho> x\<^sub>p = Some \<lbrace>prim.Pair x\<^sub>1 x\<^sub>2, \<rho>\<^sub>p\<rbrace> \<Longrightarrow> \<rho>\<^sub>p x\<^sub>1 = Some \<omega> \<Longrightarrow> (\<V>, \<C>, \<X>) \<Turnstile>\<^sub>\<kappa>  \<V> (\<lfloor>e\<rfloor>) \<Rrightarrow> \<kappa>
 "
  apply (erule accept_state.cases, auto)
 done
 
 lemma flow_over_state_6: "
-  (\<V>, \<C>) \<Turnstile>\<^sub>\<sigma>  \<langle>LET x = FST x\<^sub>p in e; \<rho>; \<kappa>\<rangle> \<Longrightarrow>
+  (\<V>, \<C>, \<X>) \<Turnstile>\<^sub>\<sigma>  \<langle>LET x = FST x\<^sub>p in e; \<rho>; \<kappa>\<rangle> \<Longrightarrow>
   \<rho> x\<^sub>p = Some \<lbrace>prim.Pair x\<^sub>1 x\<^sub>2, \<rho>\<^sub>p\<rbrace> \<Longrightarrow> \<rho>\<^sub>p x\<^sub>1 = Some \<omega> \<Longrightarrow> 
-  (\<V>, \<C>) \<Turnstile>\<^sub>\<sigma>  \<langle>e; \<rho>(x \<mapsto> \<omega>); \<kappa>\<rangle>
+  (\<V>, \<C>, \<X>) \<Turnstile>\<^sub>\<sigma>  \<langle>e; \<rho>(x \<mapsto> \<omega>); \<kappa>\<rangle>
 "
  apply (rule accept_state.Any)
     apply (erule flow_state_to_flow_exp_6, simp, auto)
@@ -305,15 +305,15 @@ lemma flow_over_state_6: "
 done
 
 lemma flow_state_to_flow_exp_7: "
-  (\<V>, \<C>) \<Turnstile>\<^sub>\<sigma>  \<langle>LET x = SND x\<^sub>p in e; \<rho>; \<kappa>\<rangle> \<Longrightarrow> \<rho> x\<^sub>p = Some \<lbrace>prim.Pair x\<^sub>1 x\<^sub>2, \<rho>\<^sub>p\<rbrace> \<Longrightarrow> 
-  \<rho>\<^sub>p x\<^sub>2 = Some \<omega> \<Longrightarrow> (\<V>, \<C>) \<Turnstile>\<^sub>e  e
+  (\<V>, \<C>, \<X>) \<Turnstile>\<^sub>\<sigma>  \<langle>LET x = SND x\<^sub>p in e; \<rho>; \<kappa>\<rangle> \<Longrightarrow> \<rho> x\<^sub>p = Some \<lbrace>prim.Pair x\<^sub>1 x\<^sub>2, \<rho>\<^sub>p\<rbrace> \<Longrightarrow> 
+  \<rho>\<^sub>p x\<^sub>2 = Some \<omega> \<Longrightarrow> (\<V>, \<C>, \<X>) \<Turnstile>\<^sub>e  e
 "
  apply (erule accept_state.cases, auto)
  apply (erule accept_exp.cases, auto)
 done
 
 lemma flow_state_to_flow_env_7: "
-  (\<V>, \<C>) \<Turnstile>\<^sub>\<sigma>  \<langle>LET x = SND x\<^sub>p in e; \<rho>; \<kappa>\<rangle> \<Longrightarrow> \<rho> x\<^sub>p = Some \<lbrace>prim.Pair x\<^sub>1 x\<^sub>2, \<rho>\<^sub>p\<rbrace> \<Longrightarrow> \<rho>\<^sub>p x\<^sub>2 = Some \<omega> \<Longrightarrow> (\<V>, \<C>) \<Turnstile>\<^sub>\<rho> \<rho>(x \<mapsto> \<omega>)
+  (\<V>, \<C>, \<X>) \<Turnstile>\<^sub>\<sigma>  \<langle>LET x = SND x\<^sub>p in e; \<rho>; \<kappa>\<rangle> \<Longrightarrow> \<rho> x\<^sub>p = Some \<lbrace>prim.Pair x\<^sub>1 x\<^sub>2, \<rho>\<^sub>p\<rbrace> \<Longrightarrow> \<rho>\<^sub>p x\<^sub>2 = Some \<omega> \<Longrightarrow> (\<V>, \<C>, \<X>) \<Turnstile>\<^sub>\<rho> \<rho>(x \<mapsto> \<omega>)
 "
  apply (rule accept_value_accept_val_env.Any, auto)
       apply (erule accept_state.cases, auto)
@@ -337,15 +337,15 @@ lemma flow_state_to_flow_env_7: "
 done
 
 lemma flow_state_to_flow_stack_7: "
-  (\<V>, \<C>) \<Turnstile>\<^sub>\<sigma>  \<langle>LET x = SND x\<^sub>p in e; \<rho>; \<kappa>\<rangle> \<Longrightarrow> \<rho> x\<^sub>p = Some \<lbrace>prim.Pair x\<^sub>1 x\<^sub>2, \<rho>\<^sub>p\<rbrace> \<Longrightarrow> \<rho>\<^sub>p x\<^sub>2 = Some \<omega> \<Longrightarrow> (\<V>, \<C>) \<Turnstile>\<^sub>\<kappa>  \<V> (\<lfloor>e\<rfloor>) \<Rrightarrow> \<kappa>
+  (\<V>, \<C>, \<X>) \<Turnstile>\<^sub>\<sigma>  \<langle>LET x = SND x\<^sub>p in e; \<rho>; \<kappa>\<rangle> \<Longrightarrow> \<rho> x\<^sub>p = Some \<lbrace>prim.Pair x\<^sub>1 x\<^sub>2, \<rho>\<^sub>p\<rbrace> \<Longrightarrow> \<rho>\<^sub>p x\<^sub>2 = Some \<omega> \<Longrightarrow> (\<V>, \<C>, \<X>) \<Turnstile>\<^sub>\<kappa>  \<V> (\<lfloor>e\<rfloor>) \<Rrightarrow> \<kappa>
 "
  apply (erule accept_state.cases, auto)
 done
 
 lemma flow_over_state_7: "
-  (\<V>, \<C>) \<Turnstile>\<^sub>\<sigma>  \<langle>LET x = SND x\<^sub>p in e; \<rho>; \<kappa>\<rangle> \<Longrightarrow>
+  (\<V>, \<C>, \<X>) \<Turnstile>\<^sub>\<sigma>  \<langle>LET x = SND x\<^sub>p in e; \<rho>; \<kappa>\<rangle> \<Longrightarrow>
   \<rho> x\<^sub>p = Some \<lbrace>prim.Pair x\<^sub>1 x\<^sub>2, \<rho>\<^sub>p\<rbrace> \<Longrightarrow> \<rho>\<^sub>p x\<^sub>2 = Some \<omega> \<Longrightarrow> 
-  (\<V>, \<C>) \<Turnstile>\<^sub>\<sigma>  \<langle>e; \<rho>(x \<mapsto> \<omega>); \<kappa>\<rangle>
+  (\<V>, \<C>, \<X>) \<Turnstile>\<^sub>\<sigma>  \<langle>e; \<rho>(x \<mapsto> \<omega>); \<kappa>\<rangle>
 "
  apply (rule accept_state.Any)
     apply (erule flow_state_to_flow_exp_7, simp, auto)
@@ -354,9 +354,9 @@ lemma flow_over_state_7: "
 done
 
 lemma flow_state_to_flow_exp_8: "
- (\<V>, \<C>) \<Turnstile>\<^sub>\<sigma>  \<langle>LET x = APP f x\<^sub>a in e; \<rho>; \<kappa>\<rangle> \<Longrightarrow> 
+ (\<V>, \<C>, \<X>) \<Turnstile>\<^sub>\<sigma>  \<langle>LET x = APP f x\<^sub>a in e; \<rho>; \<kappa>\<rangle> \<Longrightarrow> 
  \<rho> f = Some \<lbrace>Abs f\<^sub>l x\<^sub>l e\<^sub>l, \<rho>\<^sub>l\<rbrace> \<Longrightarrow> \<rho> x\<^sub>a = Some \<omega>\<^sub>a \<Longrightarrow> 
- (\<V>, \<C>) \<Turnstile>\<^sub>e  e\<^sub>l
+ (\<V>, \<C>, \<X>) \<Turnstile>\<^sub>e  e\<^sub>l
 "
  apply (erule accept_state.cases, auto)
  apply (erule accept_exp.cases, auto)
@@ -366,9 +366,9 @@ lemma flow_state_to_flow_exp_8: "
 done
 
 lemma flow_state_to_flow_env_8: "
-  (\<V>, \<C>) \<Turnstile>\<^sub>\<sigma>  \<langle>LET x = APP f x\<^sub>a in e; \<rho>; \<kappa>\<rangle> \<Longrightarrow> 
+  (\<V>, \<C>, \<X>) \<Turnstile>\<^sub>\<sigma>  \<langle>LET x = APP f x\<^sub>a in e; \<rho>; \<kappa>\<rangle> \<Longrightarrow> 
   \<rho> f = Some \<lbrace>Abs f\<^sub>l x\<^sub>l e\<^sub>l, \<rho>\<^sub>l\<rbrace> \<Longrightarrow> \<rho> x\<^sub>a = Some \<omega>\<^sub>a \<Longrightarrow> 
-  (\<V>, \<C>) \<Turnstile>\<^sub>\<rho> \<rho>\<^sub>l(f\<^sub>l \<mapsto> \<lbrace>Abs f\<^sub>l x\<^sub>l e\<^sub>l, \<rho>\<^sub>l\<rbrace>, x\<^sub>l \<mapsto> \<omega>\<^sub>a)
+  (\<V>, \<C>, \<X>) \<Turnstile>\<^sub>\<rho> \<rho>\<^sub>l(f\<^sub>l \<mapsto> \<lbrace>Abs f\<^sub>l x\<^sub>l e\<^sub>l, \<rho>\<^sub>l\<rbrace>, x\<^sub>l \<mapsto> \<omega>\<^sub>a)
 "
  apply (rule accept_value_accept_val_env.Any, auto)
            apply (erule accept_state.cases, auto)
@@ -413,9 +413,9 @@ lemma flow_state_to_flow_env_8: "
 done
 
 lemma flow_state_to_flow_stack_8: "
-  (\<V>, \<C>) \<Turnstile>\<^sub>\<sigma>  \<langle>LET x = APP f x\<^sub>a in e; \<rho>; \<kappa>\<rangle> \<Longrightarrow> 
+  (\<V>, \<C>, \<X>) \<Turnstile>\<^sub>\<sigma>  \<langle>LET x = APP f x\<^sub>a in e; \<rho>; \<kappa>\<rangle> \<Longrightarrow> 
   \<rho> f = Some \<lbrace>Abs f\<^sub>l x\<^sub>l e\<^sub>l, \<rho>\<^sub>l\<rbrace> \<Longrightarrow> \<rho> x\<^sub>a = Some \<omega>\<^sub>a \<Longrightarrow> 
-  (\<V>, \<C>) \<Turnstile>\<^sub>\<kappa>  \<V> (\<lfloor>e\<^sub>l\<rfloor>) \<Rrightarrow> \<langle>x,e,\<rho>\<rangle> # \<kappa>
+  (\<V>, \<C>, \<X>) \<Turnstile>\<^sub>\<kappa>  \<V> (\<lfloor>e\<^sub>l\<rfloor>) \<Rrightarrow> \<langle>x,e,\<rho>\<rangle> # \<kappa>
 "
  apply (rule accept_stack.Nonempty)
     apply (erule accept_state.cases, auto) 
@@ -428,9 +428,9 @@ lemma flow_state_to_flow_stack_8: "
 done
 
 lemma flow_over_state_8: "
-  (\<V>, \<C>) \<Turnstile>\<^sub>\<sigma>  \<langle>LET x = APP f x\<^sub>a in e; \<rho>; \<kappa>\<rangle> \<Longrightarrow>
+  (\<V>, \<C>, \<X>) \<Turnstile>\<^sub>\<sigma>  \<langle>LET x = APP f x\<^sub>a in e; \<rho>; \<kappa>\<rangle> \<Longrightarrow>
   \<rho> f = Some \<lbrace>Abs f\<^sub>l x\<^sub>l e\<^sub>l, \<rho>\<^sub>l\<rbrace> \<Longrightarrow> \<rho> x\<^sub>a = Some \<omega>\<^sub>a \<Longrightarrow> 
-  (\<V>, \<C>) \<Turnstile>\<^sub>\<sigma>  \<langle>e\<^sub>l; \<rho>\<^sub>l(f\<^sub>l \<mapsto> \<lbrace>Abs f\<^sub>l x\<^sub>l e\<^sub>l, \<rho>\<^sub>l\<rbrace>, x\<^sub>l \<mapsto> \<omega>\<^sub>a); \<langle>x,e,\<rho>\<rangle> # \<kappa>\<rangle>
+  (\<V>, \<C>, \<X>) \<Turnstile>\<^sub>\<sigma>  \<langle>e\<^sub>l; \<rho>\<^sub>l(f\<^sub>l \<mapsto> \<lbrace>Abs f\<^sub>l x\<^sub>l e\<^sub>l, \<rho>\<^sub>l\<rbrace>, x\<^sub>l \<mapsto> \<omega>\<^sub>a); \<langle>x,e,\<rho>\<rangle> # \<kappa>\<rangle>
 "
  apply (rule accept_state.Any)
     apply (erule flow_state_to_flow_exp_8, simp, auto)
@@ -440,10 +440,10 @@ done
 
 theorem flow_over_state_preservation : "
   \<lbrakk>
-    (\<V>, \<C>) \<Turnstile>\<^sub>\<sigma>  \<sigma>; 
+    (\<V>, \<C>, \<X>) \<Turnstile>\<^sub>\<sigma>  \<sigma>; 
     \<sigma> \<hookrightarrow> \<sigma>'
   \<rbrakk> \<Longrightarrow>
-  (\<V>, \<C>) \<Turnstile>\<^sub>\<sigma>  \<sigma>'
+  (\<V>, \<C>, \<X>) \<Turnstile>\<^sub>\<sigma>  \<sigma>'
 "
  apply (erule seq_step.cases, auto)
         apply (erule flow_over_state_1, auto)
@@ -457,8 +457,8 @@ theorem flow_over_state_preservation : "
 done
 
 lemma flow_seq_step_preservation: "
-  (\<V>, \<C>) \<Turnstile>\<^sub>\<E> \<E> \<Longrightarrow> leaf \<E> \<pi> \<Longrightarrow> \<E> \<pi> = Some (\<langle>LET x = b in e; \<rho>; \<kappa>\<rangle>) \<Longrightarrow> 
-  \<langle>LET x = b in e; \<rho>; \<kappa>\<rangle> \<hookrightarrow> \<sigma>' \<Longrightarrow> (\<V>, \<C>) \<Turnstile>\<^sub>\<E> \<E>(\<pi> ;; x \<mapsto> \<sigma>')
+  (\<V>, \<C>, \<X>) \<Turnstile>\<^sub>\<E> \<E> \<Longrightarrow> leaf \<E> \<pi> \<Longrightarrow> \<E> \<pi> = Some (\<langle>LET x = b in e; \<rho>; \<kappa>\<rangle>) \<Longrightarrow> 
+  \<langle>LET x = b in e; \<rho>; \<kappa>\<rangle> \<hookrightarrow> \<sigma>' \<Longrightarrow> (\<V>, \<C>, \<X>) \<Turnstile>\<^sub>\<E> \<E>(\<pi> ;; x \<mapsto> \<sigma>')
 "
  apply (rule accept_state_pool.Any, auto)
   apply (erule accept_state_pool.cases, auto)
@@ -468,9 +468,9 @@ lemma flow_seq_step_preservation: "
 done
 
 lemma flow_over_pool_to_exp_1: "
-  (\<V>, \<C>) \<Turnstile>\<^sub>\<E> \<E> \<Longrightarrow>
+  (\<V>, \<C>, \<X>) \<Turnstile>\<^sub>\<E> \<E> \<Longrightarrow>
   \<E> \<pi>\<^sub>s = Some (\<langle>LET x\<^sub>s = SYNC x\<^sub>s\<^sub>e in e\<^sub>s; \<rho>\<^sub>s; \<kappa>\<^sub>s\<rangle>) \<Longrightarrow>
-  (\<V>, \<C>) \<Turnstile>\<^sub>e e\<^sub>s
+  (\<V>, \<C>, \<X>) \<Turnstile>\<^sub>e e\<^sub>s
 "
  apply (erule accept_state_pool.cases, auto)
  apply (drule spec[of _ \<pi>\<^sub>s])
@@ -480,14 +480,14 @@ lemma flow_over_pool_to_exp_1: "
 done
 
 lemma flow_over_pool_to_env_1: "
-  (\<V>, \<C>) \<Turnstile>\<^sub>\<E> \<E> \<Longrightarrow>
+  (\<V>, \<C>, \<X>) \<Turnstile>\<^sub>\<E> \<E> \<Longrightarrow>
   \<E> \<pi>\<^sub>s = Some (\<langle>LET x\<^sub>s = SYNC x\<^sub>s\<^sub>e in e\<^sub>s; \<rho>\<^sub>s; \<kappa>\<^sub>s\<rangle>) \<Longrightarrow>
   \<rho>\<^sub>s x\<^sub>s\<^sub>e = Some \<lbrace>Send_Evt x\<^sub>s\<^sub>c x\<^sub>m, \<rho>\<^sub>s\<^sub>e\<rbrace> \<Longrightarrow>
   \<rho>\<^sub>s\<^sub>e x\<^sub>s\<^sub>c = Some \<lbrace>c\<rbrace> \<Longrightarrow>
   \<E> \<pi>\<^sub>r = Some (\<langle>LET x\<^sub>r = SYNC x\<^sub>r\<^sub>e in e\<^sub>r; \<rho>\<^sub>r; \<kappa>\<^sub>r\<rangle>) \<Longrightarrow>
   \<rho>\<^sub>r x\<^sub>r\<^sub>e = Some \<lbrace>Recv_Evt x\<^sub>r\<^sub>c, \<rho>\<^sub>r\<^sub>e\<rbrace> \<Longrightarrow>
   \<rho>\<^sub>r\<^sub>e x\<^sub>r\<^sub>c = Some \<lbrace>c\<rbrace> \<Longrightarrow>
-  (\<V>, \<C>) \<Turnstile>\<^sub>\<rho> \<rho>\<^sub>s(x\<^sub>s \<mapsto> \<lbrace>\<rbrace>)
+  (\<V>, \<C>, \<X>) \<Turnstile>\<^sub>\<rho> \<rho>\<^sub>s(x\<^sub>s \<mapsto> \<lbrace>\<rbrace>)
 "
 apply (rule accept_value_accept_val_env.Any; auto)
     apply (erule accept_state_pool.cases, auto)
@@ -497,22 +497,22 @@ apply (rule accept_value_accept_val_env.Any; auto)
     apply (drule spec[of _ "\<langle>LET x\<^sub>r = SYNC x\<^sub>r\<^sub>e in e\<^sub>r; \<rho>\<^sub>r; \<kappa>\<^sub>r\<rangle>"])
     apply (drule mp[of "\<E> \<pi>\<^sub>s = Some (\<langle>LET x\<^sub>s = SYNC x\<^sub>s\<^sub>e in e\<^sub>s; \<rho>\<^sub>s; \<kappa>\<^sub>s\<rangle>) "])
     apply (drule mp[of "\<E> \<pi>\<^sub>r = Some (\<langle>LET x\<^sub>r = SYNC x\<^sub>r\<^sub>e in e\<^sub>r; \<rho>\<^sub>r; \<kappa>\<^sub>r\<rangle>)"], auto)
-    apply (erule accept_state.cases[of "(\<V>, \<C>)" "\<langle>LET x\<^sub>r = SYNC x\<^sub>r\<^sub>e in e\<^sub>r; \<rho>\<^sub>r; \<kappa>\<^sub>r\<rangle>"], auto)
-    apply (erule accept_state.cases[of "(\<V>, \<C>)" "\<langle>LET x\<^sub>s = SYNC x\<^sub>s\<^sub>e in e\<^sub>s; \<rho>\<^sub>s; \<kappa>\<^sub>s\<rangle>"], auto)
-    apply (erule accept_val_env.cases[of "(\<V>, \<C>)" "\<rho>\<^sub>r"], auto)
-    apply (erule accept_val_env.cases[of "(\<V>, \<C>)" "\<rho>\<^sub>s"], auto)
+    apply (erule accept_state.cases[of "(\<V>, \<C>, \<X>)" "\<langle>LET x\<^sub>r = SYNC x\<^sub>r\<^sub>e in e\<^sub>r; \<rho>\<^sub>r; \<kappa>\<^sub>r\<rangle>"], auto)
+    apply (erule accept_state.cases[of "(\<V>, \<C>, \<X>)" "\<langle>LET x\<^sub>s = SYNC x\<^sub>s\<^sub>e in e\<^sub>s; \<rho>\<^sub>s; \<kappa>\<^sub>s\<rangle>"], auto)
+    apply (erule accept_val_env.cases[of "(\<V>, \<C>, \<X>)" "\<rho>\<^sub>r"], auto)
+    apply (erule accept_val_env.cases[of "(\<V>, \<C>, \<X>)" "\<rho>\<^sub>s"], auto)
     apply (drule spec[of _ x\<^sub>r\<^sub>e])
     apply (drule spec[of _ x\<^sub>s\<^sub>e])
     apply (drule spec[of _ "\<lbrace>Recv_Evt x\<^sub>r\<^sub>c, \<rho>\<^sub>r\<^sub>e\<rbrace>"])
     apply (drule spec[of _ "\<lbrace>Send_Evt x\<^sub>s\<^sub>c x\<^sub>m, \<rho>\<^sub>s\<^sub>e\<rbrace>"])
     apply (drule mp[of "\<rho>\<^sub>r x\<^sub>r\<^sub>e = Some \<lbrace>Recv_Evt x\<^sub>r\<^sub>c, \<rho>\<^sub>r\<^sub>e\<rbrace>"], simp)
     apply (drule mp[of "\<rho>\<^sub>s x\<^sub>s\<^sub>e = Some \<lbrace>Send_Evt x\<^sub>s\<^sub>c x\<^sub>m, \<rho>\<^sub>s\<^sub>e\<rbrace>"]; auto)
-    apply (erule accept_value.cases[of "(\<V>, \<C>)" "\<lbrace>Recv_Evt x\<^sub>r\<^sub>c, \<rho>\<^sub>r\<^sub>e\<rbrace>"]; auto)
-    apply (erule accept_value.cases[of "(\<V>, \<C>)" "\<lbrace>Send_Evt x\<^sub>s\<^sub>c x\<^sub>m, \<rho>\<^sub>s\<^sub>e\<rbrace> "]; auto)
-    apply (erule accept_val_env.cases[of "(\<V>, \<C>)" "\<rho>\<^sub>r\<^sub>e"], auto)
-    apply (erule accept_val_env.cases[of "(\<V>, \<C>)" "\<rho>\<^sub>s\<^sub>e"], auto)
-    apply (erule accept_exp.cases[of "(\<V>, \<C>)" "LET x\<^sub>r = SYNC x\<^sub>r\<^sub>e in e\<^sub>r"]; auto)
-    apply (erule accept_exp.cases[of "(\<V>, \<C>)" "LET x\<^sub>s = SYNC x\<^sub>s\<^sub>e in e\<^sub>s"]; auto)
+    apply (erule accept_value.cases[of "(\<V>, \<C>, \<X>)" "\<lbrace>Recv_Evt x\<^sub>r\<^sub>c, \<rho>\<^sub>r\<^sub>e\<rbrace>"]; auto)
+    apply (erule accept_value.cases[of "(\<V>, \<C>, \<X>)" "\<lbrace>Send_Evt x\<^sub>s\<^sub>c x\<^sub>m, \<rho>\<^sub>s\<^sub>e\<rbrace> "]; auto)
+    apply (erule accept_val_env.cases[of "(\<V>, \<C>, \<X>)" "\<rho>\<^sub>r\<^sub>e"], auto)
+    apply (erule accept_val_env.cases[of "(\<V>, \<C>, \<X>)" "\<rho>\<^sub>s\<^sub>e"], auto)
+    apply (erule accept_exp.cases[of "(\<V>, \<C>, \<X>)" "LET x\<^sub>r = SYNC x\<^sub>r\<^sub>e in e\<^sub>r"]; auto)
+    apply (erule accept_exp.cases[of "(\<V>, \<C>, \<X>)" "LET x\<^sub>s = SYNC x\<^sub>s\<^sub>e in e\<^sub>s"]; auto)
     apply (thin_tac "\<forall>x\<^sub>s\<^sub>c x\<^sub>m. ^Send_Evt x\<^sub>s\<^sub>c x\<^sub>m \<in> \<V> x\<^sub>r\<^sub>e \<longrightarrow> (\<forall>x\<^sub>c. ^Chan x\<^sub>c \<in> \<V> x\<^sub>s\<^sub>c \<longrightarrow> ^\<lparr>\<rparr> \<in> \<V> x\<^sub>r \<and> \<V> x\<^sub>m \<subseteq> \<C> x\<^sub>c)")
     apply (thin_tac "\<forall>x\<^sub>r\<^sub>c. ^Recv_Evt x\<^sub>r\<^sub>c \<in> \<V> x\<^sub>s\<^sub>e \<longrightarrow> (\<forall>x\<^sub>c. ^Chan x\<^sub>c \<in> \<V> x\<^sub>r\<^sub>c \<longrightarrow> \<C> x\<^sub>c \<subseteq> \<V> x\<^sub>s)")
     apply (drule spec[of _ x\<^sub>r\<^sub>c])
@@ -534,9 +534,9 @@ apply (rule accept_value_accept_val_env.Any; auto)
 done
 
 lemma flow_over_pool_to_stack_1: "
-  (\<V>, \<C>) \<Turnstile>\<^sub>\<E> \<E> \<Longrightarrow>
+  (\<V>, \<C>, \<X>) \<Turnstile>\<^sub>\<E> \<E> \<Longrightarrow>
   \<E> \<pi>\<^sub>s = Some (\<langle>LET x\<^sub>s = SYNC x\<^sub>s\<^sub>e in e\<^sub>s; \<rho>\<^sub>s; \<kappa>\<^sub>s\<rangle>) \<Longrightarrow>
-  (\<V>, \<C>) \<Turnstile>\<^sub>\<kappa>  \<V> (\<lfloor>e\<^sub>s\<rfloor>) \<Rrightarrow> \<kappa>\<^sub>s
+  (\<V>, \<C>, \<X>) \<Turnstile>\<^sub>\<kappa>  \<V> (\<lfloor>e\<^sub>s\<rfloor>) \<Rrightarrow> \<kappa>\<^sub>s
 "
  apply (erule accept_state_pool.cases, auto)
  apply (drule spec[of _ \<pi>\<^sub>s])
@@ -545,9 +545,9 @@ lemma flow_over_pool_to_stack_1: "
 done
 
 lemma flow_over_pool_to_exp_2: "
-  (\<V>, \<C>) \<Turnstile>\<^sub>\<E> \<E> \<Longrightarrow>
+  (\<V>, \<C>, \<X>) \<Turnstile>\<^sub>\<E> \<E> \<Longrightarrow>
   \<E> \<pi>\<^sub>r = Some (\<langle>LET x\<^sub>r = SYNC x\<^sub>r\<^sub>e in e\<^sub>r; \<rho>\<^sub>r; \<kappa>\<^sub>r\<rangle>) \<Longrightarrow> 
-  (\<V>, \<C>) \<Turnstile>\<^sub>e  e\<^sub>r
+  (\<V>, \<C>, \<X>) \<Turnstile>\<^sub>e  e\<^sub>r
 "
  apply (erule accept_state_pool.cases, auto)
  apply (drule spec[of _ \<pi>\<^sub>r])
@@ -557,7 +557,7 @@ lemma flow_over_pool_to_exp_2: "
 done
 
 lemma flow_over_pool_to_env_2: "
-  (\<V>, \<C>) \<Turnstile>\<^sub>\<E> \<E> \<Longrightarrow>
+  (\<V>, \<C>, \<X>) \<Turnstile>\<^sub>\<E> \<E> \<Longrightarrow>
   \<E>' = \<E>(\<pi>\<^sub>s ;; x\<^sub>s \<mapsto> \<langle>e\<^sub>s; \<rho>\<^sub>s(x\<^sub>s \<mapsto> \<lbrace>\<rbrace>); \<kappa>\<^sub>s\<rangle>, \<pi>\<^sub>r ;; x\<^sub>r \<mapsto> \<langle>e\<^sub>r; \<rho>\<^sub>r(x\<^sub>r \<mapsto> \<omega>\<^sub>m); \<kappa>\<^sub>r\<rangle>) \<Longrightarrow>
   leaf \<E> \<pi>\<^sub>s \<Longrightarrow>
   \<E> \<pi>\<^sub>s = Some (\<langle>LET x\<^sub>s = SYNC x\<^sub>s\<^sub>e in e\<^sub>s; \<rho>\<^sub>s; \<kappa>\<^sub>s\<rangle>) \<Longrightarrow>
@@ -568,7 +568,7 @@ lemma flow_over_pool_to_env_2: "
   \<E> \<pi>\<^sub>r = Some (\<langle>LET x\<^sub>r = SYNC x\<^sub>r\<^sub>e in e\<^sub>r; \<rho>\<^sub>r; \<kappa>\<^sub>r\<rangle>) \<Longrightarrow> 
   \<rho>\<^sub>r x\<^sub>r\<^sub>e = Some \<lbrace>Recv_Evt x\<^sub>r\<^sub>c, \<rho>\<^sub>r\<^sub>e\<rbrace> \<Longrightarrow> 
   \<rho>\<^sub>r\<^sub>e x\<^sub>r\<^sub>c = Some \<lbrace>c\<rbrace> \<Longrightarrow> 
-  (\<V>, \<C>) \<Turnstile>\<^sub>\<rho> \<rho>\<^sub>r(x\<^sub>r \<mapsto> \<omega>\<^sub>m)
+  (\<V>, \<C>, \<X>) \<Turnstile>\<^sub>\<rho> \<rho>\<^sub>r(x\<^sub>r \<mapsto> \<omega>\<^sub>m)
 "
 apply (rule accept_value_accept_val_env.Any; auto)
       apply (erule accept_state_pool.cases, auto)
@@ -578,22 +578,22 @@ apply (rule accept_value_accept_val_env.Any; auto)
       apply (drule spec[of _ "\<langle>LET x\<^sub>r = SYNC x\<^sub>r\<^sub>e in e\<^sub>r; \<rho>\<^sub>r; \<kappa>\<^sub>r\<rangle>"])
       apply (drule mp[of "\<E> \<pi>\<^sub>s = Some (\<langle>LET x\<^sub>s = SYNC x\<^sub>s\<^sub>e in e\<^sub>s; \<rho>\<^sub>s; \<kappa>\<^sub>s\<rangle>) "])
       apply (drule mp[of "\<E> \<pi>\<^sub>r = Some (\<langle>LET x\<^sub>r = SYNC x\<^sub>r\<^sub>e in e\<^sub>r; \<rho>\<^sub>r; \<kappa>\<^sub>r\<rangle>)"], auto)
-      apply (erule accept_state.cases[of "(\<V>, \<C>)" "\<langle>LET x\<^sub>r = SYNC x\<^sub>r\<^sub>e in e\<^sub>r; \<rho>\<^sub>r; \<kappa>\<^sub>r\<rangle>"], auto)
-      apply (erule accept_state.cases[of "(\<V>, \<C>)" "\<langle>LET x\<^sub>s = SYNC x\<^sub>s\<^sub>e in e\<^sub>s; \<rho>\<^sub>s; \<kappa>\<^sub>s\<rangle>"], auto)
-      apply (erule accept_val_env.cases[of "(\<V>, \<C>)" "\<rho>\<^sub>r"], auto)
-      apply (erule accept_val_env.cases[of "(\<V>, \<C>)" "\<rho>\<^sub>s"], auto)
+      apply (erule accept_state.cases[of "(\<V>, \<C>, \<X>)" "\<langle>LET x\<^sub>r = SYNC x\<^sub>r\<^sub>e in e\<^sub>r; \<rho>\<^sub>r; \<kappa>\<^sub>r\<rangle>"], auto)
+      apply (erule accept_state.cases[of "(\<V>, \<C>, \<X>)" "\<langle>LET x\<^sub>s = SYNC x\<^sub>s\<^sub>e in e\<^sub>s; \<rho>\<^sub>s; \<kappa>\<^sub>s\<rangle>"], auto)
+      apply (erule accept_val_env.cases[of "(\<V>, \<C>, \<X>)" "\<rho>\<^sub>r"], auto)
+      apply (erule accept_val_env.cases[of "(\<V>, \<C>, \<X>)" "\<rho>\<^sub>s"], auto)
       apply (drule spec[of _ x\<^sub>r\<^sub>e])
       apply (drule spec[of _ x\<^sub>s\<^sub>e])
       apply (drule spec[of _ "\<lbrace>Recv_Evt x\<^sub>r\<^sub>c, \<rho>\<^sub>r\<^sub>e\<rbrace>"])
       apply (drule spec[of _ "\<lbrace>Send_Evt x\<^sub>s\<^sub>c x\<^sub>m, \<rho>\<^sub>s\<^sub>e\<rbrace>"])
       apply (drule mp[of "\<rho>\<^sub>r x\<^sub>r\<^sub>e = Some \<lbrace>Recv_Evt x\<^sub>r\<^sub>c, \<rho>\<^sub>r\<^sub>e\<rbrace>"], simp)
       apply (drule mp[of "\<rho>\<^sub>s x\<^sub>s\<^sub>e = Some \<lbrace>Send_Evt x\<^sub>s\<^sub>c x\<^sub>m, \<rho>\<^sub>s\<^sub>e\<rbrace>"]; auto)
-      apply (erule accept_value.cases[of "(\<V>, \<C>)" "\<lbrace>Recv_Evt x\<^sub>r\<^sub>c, \<rho>\<^sub>r\<^sub>e\<rbrace>"]; auto)
-      apply (erule accept_value.cases[of "(\<V>, \<C>)" "\<lbrace>Send_Evt x\<^sub>s\<^sub>c x\<^sub>m, \<rho>\<^sub>s\<^sub>e\<rbrace> "]; auto)
-      apply (erule accept_val_env.cases[of "(\<V>, \<C>)" "\<rho>\<^sub>r\<^sub>e"], auto)
-      apply (erule accept_val_env.cases[of "(\<V>, \<C>)" "\<rho>\<^sub>s\<^sub>e"], auto)
-      apply (erule accept_exp.cases[of "(\<V>, \<C>)" "LET x\<^sub>r = SYNC x\<^sub>r\<^sub>e in e\<^sub>r"]; auto)
-      apply (erule accept_exp.cases[of "(\<V>, \<C>)" "LET x\<^sub>s = SYNC x\<^sub>s\<^sub>e in e\<^sub>s"]; auto)
+      apply (erule accept_value.cases[of "(\<V>, \<C>, \<X>)" "\<lbrace>Recv_Evt x\<^sub>r\<^sub>c, \<rho>\<^sub>r\<^sub>e\<rbrace>"]; auto)
+      apply (erule accept_value.cases[of "(\<V>, \<C>, \<X>)" "\<lbrace>Send_Evt x\<^sub>s\<^sub>c x\<^sub>m, \<rho>\<^sub>s\<^sub>e\<rbrace> "]; auto)
+      apply (erule accept_val_env.cases[of "(\<V>, \<C>, \<X>)" "\<rho>\<^sub>r\<^sub>e"], auto)
+      apply (erule accept_val_env.cases[of "(\<V>, \<C>, \<X>)" "\<rho>\<^sub>s\<^sub>e"], auto)
+      apply (erule accept_exp.cases[of "(\<V>, \<C>, \<X>)" "LET x\<^sub>r = SYNC x\<^sub>r\<^sub>e in e\<^sub>r"]; auto)
+      apply (erule accept_exp.cases[of "(\<V>, \<C>, \<X>)" "LET x\<^sub>s = SYNC x\<^sub>s\<^sub>e in e\<^sub>s"]; auto)
       apply (thin_tac "\<forall>x\<^sub>s\<^sub>c x\<^sub>m. ^Send_Evt x\<^sub>s\<^sub>c x\<^sub>m \<in> \<V> x\<^sub>r\<^sub>e \<longrightarrow> (\<forall>x\<^sub>c. ^Chan x\<^sub>c \<in> \<V> x\<^sub>s\<^sub>c \<longrightarrow> ^\<lparr>\<rparr> \<in> \<V> x\<^sub>r \<and> \<V> x\<^sub>m \<subseteq> \<C> x\<^sub>c)")
       apply (thin_tac "\<forall>x\<^sub>r\<^sub>c. ^Recv_Evt x\<^sub>r\<^sub>c \<in> \<V> x\<^sub>s\<^sub>e \<longrightarrow> (\<forall>x\<^sub>c. ^Chan x\<^sub>c \<in> \<V> x\<^sub>r\<^sub>c \<longrightarrow> \<C> x\<^sub>c \<subseteq> \<V> x\<^sub>s)")
       apply (drule spec[of _ x\<^sub>r\<^sub>c])
@@ -611,13 +611,13 @@ apply (rule accept_value_accept_val_env.Any; auto)
     apply (drule spec[of _ \<pi>\<^sub>s])
     apply (drule spec[of _ "\<langle>LET x\<^sub>s = SYNC x\<^sub>s\<^sub>e in e\<^sub>s; \<rho>\<^sub>s; \<kappa>\<^sub>s\<rangle>"])
     apply (drule mp[of "\<E> \<pi>\<^sub>s = Some (\<langle>LET x\<^sub>s = SYNC x\<^sub>s\<^sub>e in e\<^sub>s; \<rho>\<^sub>s; \<kappa>\<^sub>s\<rangle>) "], auto)
-    apply (erule accept_state.cases[of "(\<V>, \<C>)" "\<langle>LET x\<^sub>s = SYNC x\<^sub>s\<^sub>e in e\<^sub>s; \<rho>\<^sub>s; \<kappa>\<^sub>s\<rangle>"], auto)
-    apply (erule accept_val_env.cases[of "(\<V>, \<C>)" "\<rho>\<^sub>s"], auto)
+    apply (erule accept_state.cases[of "(\<V>, \<C>, \<X>)" "\<langle>LET x\<^sub>s = SYNC x\<^sub>s\<^sub>e in e\<^sub>s; \<rho>\<^sub>s; \<kappa>\<^sub>s\<rangle>"], auto)
+    apply (erule accept_val_env.cases[of "(\<V>, \<C>, \<X>)" "\<rho>\<^sub>s"], auto)
     apply (drule spec[of _ x\<^sub>s\<^sub>e])
     apply (drule spec[of _ "\<lbrace>Send_Evt x\<^sub>s\<^sub>c x\<^sub>m, \<rho>\<^sub>s\<^sub>e\<rbrace>"])
     apply (drule mp[of "\<rho>\<^sub>s x\<^sub>s\<^sub>e = Some \<lbrace>Send_Evt x\<^sub>s\<^sub>c x\<^sub>m, \<rho>\<^sub>s\<^sub>e\<rbrace>"]; auto)
-    apply (erule accept_value.cases[of "(\<V>, \<C>)" "\<lbrace>Send_Evt x\<^sub>s\<^sub>c x\<^sub>m, \<rho>\<^sub>s\<^sub>e\<rbrace> "]; auto)
-    apply (erule accept_val_env.cases[of "(\<V>, \<C>)" "\<rho>\<^sub>s\<^sub>e"], auto)
+    apply (erule accept_value.cases[of "(\<V>, \<C>, \<X>)" "\<lbrace>Send_Evt x\<^sub>s\<^sub>c x\<^sub>m, \<rho>\<^sub>s\<^sub>e\<rbrace> "]; auto)
+    apply (erule accept_val_env.cases[of "(\<V>, \<C>, \<X>)" "\<rho>\<^sub>s\<^sub>e"], auto)
    apply (erule accept_state_pool.cases, auto)
    apply (drule spec[of _ \<pi>\<^sub>r])
    apply (drule spec[of _ "\<langle>LET x\<^sub>r = SYNC x\<^sub>r\<^sub>e in e\<^sub>r; \<rho>\<^sub>r; \<kappa>\<^sub>r\<rangle>"]; auto)
@@ -631,9 +631,9 @@ apply (rule accept_value_accept_val_env.Any; auto)
 done
 
 lemma flow_over_pool_to_stack_2: "
-  (\<V>, \<C>) \<Turnstile>\<^sub>\<E> \<E> \<Longrightarrow>
+  (\<V>, \<C>, \<X>) \<Turnstile>\<^sub>\<E> \<E> \<Longrightarrow>
   \<E> \<pi>\<^sub>r = Some (\<langle>LET x\<^sub>r = SYNC x\<^sub>r\<^sub>e in e\<^sub>r; \<rho>\<^sub>r; \<kappa>\<^sub>r\<rangle>) \<Longrightarrow>
-  (\<V>, \<C>) \<Turnstile>\<^sub>\<kappa>  \<V> (\<lfloor>e\<^sub>r\<rfloor>) \<Rrightarrow> \<kappa>\<^sub>r
+  (\<V>, \<C>, \<X>) \<Turnstile>\<^sub>\<kappa>  \<V> (\<lfloor>e\<^sub>r\<rfloor>) \<Rrightarrow> \<kappa>\<^sub>r
 "
  apply (erule accept_state_pool.cases, auto)
  apply (drule spec[of _ \<pi>\<^sub>r])
@@ -642,7 +642,7 @@ lemma flow_over_pool_to_stack_2: "
 done
 
 lemma flow_let_sync_preservation: "
-  (\<V>, \<C>) \<Turnstile>\<^sub>\<E> \<E> \<Longrightarrow>
+  (\<V>, \<C>, \<X>) \<Turnstile>\<^sub>\<E> \<E> \<Longrightarrow>
   \<E>' = \<E>(\<pi>\<^sub>s ;; x\<^sub>s \<mapsto> \<langle>e\<^sub>s; \<rho>\<^sub>s(x\<^sub>s \<mapsto> \<lbrace>\<rbrace>); \<kappa>\<^sub>s\<rangle>, \<pi>\<^sub>r ;; x\<^sub>r \<mapsto> \<langle>e\<^sub>r; \<rho>\<^sub>r(x\<^sub>r \<mapsto> \<omega>\<^sub>m); \<kappa>\<^sub>r\<rangle>) \<Longrightarrow>
   leaf \<E> \<pi>\<^sub>s \<Longrightarrow>
   \<E> \<pi>\<^sub>s = Some (\<langle>LET x\<^sub>s = SYNC x\<^sub>s\<^sub>e in e\<^sub>s; \<rho>\<^sub>s; \<kappa>\<^sub>s\<rangle>) \<Longrightarrow>
@@ -652,7 +652,7 @@ lemma flow_let_sync_preservation: "
   leaf \<E> \<pi>\<^sub>r \<Longrightarrow>
   \<E> \<pi>\<^sub>r = Some (\<langle>LET x\<^sub>r = SYNC x\<^sub>r\<^sub>e in e\<^sub>r; \<rho>\<^sub>r; \<kappa>\<^sub>r\<rangle>) \<Longrightarrow>
   \<rho>\<^sub>r x\<^sub>r\<^sub>e = Some \<lbrace>Recv_Evt x\<^sub>r\<^sub>c, \<rho>\<^sub>r\<^sub>e\<rbrace> \<Longrightarrow>
-  \<rho>\<^sub>r\<^sub>e x\<^sub>r\<^sub>c = Some \<lbrace>c\<rbrace> \<Longrightarrow> (\<V>, \<C>) \<Turnstile>\<^sub>\<E> \<E>(\<pi>\<^sub>s ;; x\<^sub>s \<mapsto> \<langle>e\<^sub>s; \<rho>\<^sub>s(x\<^sub>s \<mapsto> \<lbrace>\<rbrace>); \<kappa>\<^sub>s\<rangle>, \<pi>\<^sub>r ;; x\<^sub>r \<mapsto> \<langle>e\<^sub>r; \<rho>\<^sub>r(x\<^sub>r \<mapsto> \<omega>\<^sub>m); \<kappa>\<^sub>r\<rangle>)
+  \<rho>\<^sub>r\<^sub>e x\<^sub>r\<^sub>c = Some \<lbrace>c\<rbrace> \<Longrightarrow> (\<V>, \<C>, \<X>) \<Turnstile>\<^sub>\<E> \<E>(\<pi>\<^sub>s ;; x\<^sub>s \<mapsto> \<langle>e\<^sub>s; \<rho>\<^sub>s(x\<^sub>s \<mapsto> \<lbrace>\<rbrace>); \<kappa>\<^sub>s\<rangle>, \<pi>\<^sub>r ;; x\<^sub>r \<mapsto> \<langle>e\<^sub>r; \<rho>\<^sub>r(x\<^sub>r \<mapsto> \<omega>\<^sub>m); \<kappa>\<^sub>r\<rangle>)
 "
  apply (rule accept_state_pool.Any, auto)
      apply (rule accept_state.Any)
@@ -677,9 +677,9 @@ lemma flow_let_sync_preservation: "
 done
 
 lemma flow_over_pool_to_exp_3: "
-  (\<V>, \<C>) \<Turnstile>\<^sub>\<E> \<E> \<Longrightarrow> \<E>' = \<E>(\<pi> ;; x \<mapsto> \<langle>e; \<rho>(x \<mapsto> \<lbrace>Ch \<pi> x\<rbrace>); \<kappa>\<rangle>) \<Longrightarrow> 
+  (\<V>, \<C>, \<X>) \<Turnstile>\<^sub>\<E> \<E> \<Longrightarrow> \<E>' = \<E>(\<pi> ;; x \<mapsto> \<langle>e; \<rho>(x \<mapsto> \<lbrace>Ch \<pi> x\<rbrace>); \<kappa>\<rangle>) \<Longrightarrow> 
   leaf \<E> \<pi> \<Longrightarrow> \<E> \<pi> = Some (\<langle>LET x = CHAN \<lparr>\<rparr> in e; \<rho>; \<kappa>\<rangle>) \<Longrightarrow> 
-  (\<V>, \<C>) \<Turnstile>\<^sub>e  e
+  (\<V>, \<C>, \<X>) \<Turnstile>\<^sub>e  e
 "
  apply (erule accept_state_pool.cases, auto)
  apply (drule spec[of _ \<pi>])
@@ -689,9 +689,9 @@ lemma flow_over_pool_to_exp_3: "
 done
 
 lemma flow_over_pool_to_env_3: "
-  (\<V>, \<C>) \<Turnstile>\<^sub>\<E> \<E> \<Longrightarrow> \<E>' = \<E>(\<pi> ;; x \<mapsto> \<langle>e; \<rho>(x \<mapsto> \<lbrace>Ch \<pi> x\<rbrace>); \<kappa>\<rangle>) \<Longrightarrow> 
+  (\<V>, \<C>, \<X>) \<Turnstile>\<^sub>\<E> \<E> \<Longrightarrow> \<E>' = \<E>(\<pi> ;; x \<mapsto> \<langle>e; \<rho>(x \<mapsto> \<lbrace>Ch \<pi> x\<rbrace>); \<kappa>\<rangle>) \<Longrightarrow> 
   leaf \<E> \<pi> \<Longrightarrow> \<E> \<pi> = Some (\<langle>LET x = CHAN \<lparr>\<rparr> in e; \<rho>; \<kappa>\<rangle>) \<Longrightarrow> 
-  (\<V>, \<C>) \<Turnstile>\<^sub>\<rho> \<rho>(x \<mapsto> \<lbrace>Ch \<pi> x\<rbrace>)
+  (\<V>, \<C>, \<X>) \<Turnstile>\<^sub>\<rho> \<rho>(x \<mapsto> \<lbrace>Ch \<pi> x\<rbrace>)
 "
  apply (rule accept_value_accept_val_env.Any, auto)
       apply (erule accept_state_pool.cases, auto)
@@ -717,7 +717,7 @@ lemma flow_over_pool_to_env_3: "
 done
 
 lemma flow_over_pool_to_stack_3: "
-  (\<V>, \<C>) \<Turnstile>\<^sub>\<E> \<E> \<Longrightarrow> \<E>' = \<E>(\<pi> ;; x \<mapsto> \<langle>e; \<rho>(x \<mapsto> \<lbrace>Ch \<pi> x\<rbrace>); \<kappa>\<rangle>) \<Longrightarrow> leaf \<E> \<pi> \<Longrightarrow> \<E> \<pi> = Some (\<langle>LET x = CHAN \<lparr>\<rparr> in e; \<rho>; \<kappa>\<rangle>) \<Longrightarrow> (\<V>, \<C>) \<Turnstile>\<^sub>\<kappa>  \<V> (\<lfloor>e\<rfloor>) \<Rrightarrow> \<kappa>
+  (\<V>, \<C>, \<X>) \<Turnstile>\<^sub>\<E> \<E> \<Longrightarrow> \<E>' = \<E>(\<pi> ;; x \<mapsto> \<langle>e; \<rho>(x \<mapsto> \<lbrace>Ch \<pi> x\<rbrace>); \<kappa>\<rangle>) \<Longrightarrow> leaf \<E> \<pi> \<Longrightarrow> \<E> \<pi> = Some (\<langle>LET x = CHAN \<lparr>\<rparr> in e; \<rho>; \<kappa>\<rangle>) \<Longrightarrow> (\<V>, \<C>, \<X>) \<Turnstile>\<^sub>\<kappa>  \<V> (\<lfloor>e\<rfloor>) \<Rrightarrow> \<kappa>
 "
  apply (erule accept_state_pool.cases, auto)
  apply (drule spec[of _ \<pi>])
@@ -726,9 +726,9 @@ lemma flow_over_pool_to_stack_3: "
 done
 
 lemma flow_over_pool_to_exp_4: "
-  (\<V>, \<C>) \<Turnstile>\<^sub>\<E> \<E> \<Longrightarrow> \<E>' = \<E>(\<pi> ;; x \<mapsto> \<langle>e; \<rho>(x \<mapsto> \<lbrace>Ch \<pi> x\<rbrace>); \<kappa>\<rangle>) \<Longrightarrow>
+  (\<V>, \<C>, \<X>) \<Turnstile>\<^sub>\<E> \<E> \<Longrightarrow> \<E>' = \<E>(\<pi> ;; x \<mapsto> \<langle>e; \<rho>(x \<mapsto> \<lbrace>Ch \<pi> x\<rbrace>); \<kappa>\<rangle>) \<Longrightarrow>
   leaf \<E> \<pi> \<Longrightarrow> \<E> \<pi> = Some (\<langle>LET x = CHAN \<lparr>\<rparr> in e; \<rho>; \<kappa>\<rangle>) \<Longrightarrow> \<pi>' \<noteq> \<pi> ;; x \<Longrightarrow> \<E> \<pi>' = Some (\<langle>e'; \<rho>'; \<kappa>'\<rangle>) \<Longrightarrow> 
-  (\<V>, \<C>) \<Turnstile>\<^sub>e  e'
+  (\<V>, \<C>, \<X>) \<Turnstile>\<^sub>e  e'
 "
  apply (erule accept_state_pool.cases, auto)
  apply (drule spec[of _ \<pi>'])
@@ -737,9 +737,9 @@ lemma flow_over_pool_to_exp_4: "
 done
 
 lemma flow_over_pool_to_env_4: "
-  (\<V>, \<C>) \<Turnstile>\<^sub>\<E> \<E> \<Longrightarrow> \<E>' = \<E>(\<pi> ;; x \<mapsto> \<langle>e; \<rho>(x \<mapsto> \<lbrace>Ch \<pi> x\<rbrace>); \<kappa>\<rangle>) \<Longrightarrow>
+  (\<V>, \<C>, \<X>) \<Turnstile>\<^sub>\<E> \<E> \<Longrightarrow> \<E>' = \<E>(\<pi> ;; x \<mapsto> \<langle>e; \<rho>(x \<mapsto> \<lbrace>Ch \<pi> x\<rbrace>); \<kappa>\<rangle>) \<Longrightarrow>
   leaf \<E> \<pi> \<Longrightarrow> \<E> \<pi> = Some (\<langle>LET x = CHAN \<lparr>\<rparr> in e; \<rho>; \<kappa>\<rangle>) \<Longrightarrow> \<pi>' \<noteq> \<pi> ;; x \<Longrightarrow> \<E> \<pi>' = Some (\<langle>e'; \<rho>'; \<kappa>'\<rangle>) \<Longrightarrow> 
-  (\<V>, \<C>) \<Turnstile>\<^sub>\<rho> \<rho>'
+  (\<V>, \<C>, \<X>) \<Turnstile>\<^sub>\<rho> \<rho>'
 "
  apply (rule accept_value_accept_val_env.Any, auto)
     apply (erule accept_state_pool.cases, auto)
@@ -755,9 +755,9 @@ lemma flow_over_pool_to_env_4: "
 done
 
 lemma flow_over_pool_to_stack_4: "
-  (\<V>, \<C>) \<Turnstile>\<^sub>\<E> \<E> \<Longrightarrow> \<E>' = \<E>(\<pi> ;; x \<mapsto> \<langle>e; \<rho>(x \<mapsto> \<lbrace>Ch \<pi> x\<rbrace>); \<kappa>\<rangle>) \<Longrightarrow>
+  (\<V>, \<C>, \<X>) \<Turnstile>\<^sub>\<E> \<E> \<Longrightarrow> \<E>' = \<E>(\<pi> ;; x \<mapsto> \<langle>e; \<rho>(x \<mapsto> \<lbrace>Ch \<pi> x\<rbrace>); \<kappa>\<rangle>) \<Longrightarrow>
   leaf \<E> \<pi> \<Longrightarrow> \<E> \<pi> = Some (\<langle>LET x = CHAN \<lparr>\<rparr> in e; \<rho>; \<kappa>\<rangle>) \<Longrightarrow> \<pi>' \<noteq> \<pi> ;; x \<Longrightarrow> \<E> \<pi>' = Some (\<langle>e'; \<rho>'; \<kappa>'\<rangle>) \<Longrightarrow> 
-  (\<V>, \<C>) \<Turnstile>\<^sub>\<kappa>  \<V> (\<lfloor>e'\<rfloor>) \<Rrightarrow> \<kappa>'
+  (\<V>, \<C>, \<X>) \<Turnstile>\<^sub>\<kappa>  \<V> (\<lfloor>e'\<rfloor>) \<Rrightarrow> \<kappa>'
 "
  apply (erule accept_state_pool.cases, auto)
  apply (drule spec[of _ \<pi>'])
@@ -766,9 +766,9 @@ lemma flow_over_pool_to_stack_4: "
 done
 
 lemma flow_let_chan_preservation: "
-  (\<V>, \<C>) \<Turnstile>\<^sub>\<E> \<E> \<Longrightarrow> \<E>' = \<E>(\<pi> ;; x \<mapsto> \<langle>e; \<rho>(x \<mapsto> \<lbrace>Ch \<pi> x\<rbrace>); \<kappa>\<rangle>) \<Longrightarrow> 
+  (\<V>, \<C>, \<X>) \<Turnstile>\<^sub>\<E> \<E> \<Longrightarrow> \<E>' = \<E>(\<pi> ;; x \<mapsto> \<langle>e; \<rho>(x \<mapsto> \<lbrace>Ch \<pi> x\<rbrace>); \<kappa>\<rangle>) \<Longrightarrow> 
   leaf \<E> \<pi> \<Longrightarrow> \<E> \<pi> = Some (\<langle>LET x = CHAN \<lparr>\<rparr> in e; \<rho>; \<kappa>\<rangle>) \<Longrightarrow> 
-  (\<V>, \<C>) \<Turnstile>\<^sub>\<E> \<E>(\<pi> ;; x \<mapsto> \<langle>e; \<rho>(x \<mapsto> \<lbrace>Ch \<pi> x\<rbrace>); \<kappa>\<rangle>)
+  (\<V>, \<C>, \<X>) \<Turnstile>\<^sub>\<E> \<E>(\<pi> ;; x \<mapsto> \<langle>e; \<rho>(x \<mapsto> \<lbrace>Ch \<pi> x\<rbrace>); \<kappa>\<rangle>)
 "
  apply (rule accept_state_pool.Any, auto)
   apply (rule accept_state.Any)
@@ -784,9 +784,9 @@ done
 
 
 lemma flow_over_pool_to_exp_5: "
-  (\<V>, \<C>) \<Turnstile>\<^sub>\<E> \<E> \<Longrightarrow> \<E>' = \<E>(\<pi> ;; x \<mapsto> \<langle>e; \<rho>(x \<mapsto> \<lbrace>\<rbrace>); \<kappa>\<rangle>, \<pi>;;. \<mapsto> \<langle>e\<^sub>c; \<rho>; []\<rangle>) \<Longrightarrow> 
+  (\<V>, \<C>, \<X>) \<Turnstile>\<^sub>\<E> \<E> \<Longrightarrow> \<E>' = \<E>(\<pi> ;; x \<mapsto> \<langle>e; \<rho>(x \<mapsto> \<lbrace>\<rbrace>); \<kappa>\<rangle>, \<pi>;;. \<mapsto> \<langle>e\<^sub>c; \<rho>; []\<rangle>) \<Longrightarrow> 
   leaf \<E> \<pi> \<Longrightarrow> \<E> \<pi> = Some (\<langle>LET x = SPAWN e\<^sub>c in e; \<rho>; \<kappa>\<rangle>) \<Longrightarrow> 
-  (\<V>, \<C>) \<Turnstile>\<^sub>e  e
+  (\<V>, \<C>, \<X>) \<Turnstile>\<^sub>e  e
 "
  apply (erule accept_state_pool.cases, auto)
  apply (drule spec[of _ \<pi>])
@@ -796,9 +796,9 @@ lemma flow_over_pool_to_exp_5: "
 done
 
 lemma flow_over_pool_to_env_5: "
-  (\<V>, \<C>) \<Turnstile>\<^sub>\<E> \<E> \<Longrightarrow> \<E>' = \<E>(\<pi> ;; x \<mapsto> \<langle>e; \<rho>(x \<mapsto> \<lbrace>\<rbrace>); \<kappa>\<rangle>, \<pi>;;. \<mapsto> \<langle>e\<^sub>c; \<rho>; []\<rangle>) \<Longrightarrow> 
+  (\<V>, \<C>, \<X>) \<Turnstile>\<^sub>\<E> \<E> \<Longrightarrow> \<E>' = \<E>(\<pi> ;; x \<mapsto> \<langle>e; \<rho>(x \<mapsto> \<lbrace>\<rbrace>); \<kappa>\<rangle>, \<pi>;;. \<mapsto> \<langle>e\<^sub>c; \<rho>; []\<rangle>) \<Longrightarrow> 
   leaf \<E> \<pi> \<Longrightarrow> \<E> \<pi> = Some (\<langle>LET x = SPAWN e\<^sub>c in e; \<rho>; \<kappa>\<rangle>) \<Longrightarrow> 
-  (\<V>, \<C>) \<Turnstile>\<^sub>\<rho> \<rho>(x \<mapsto> \<lbrace>\<rbrace>)"
+  (\<V>, \<C>, \<X>) \<Turnstile>\<^sub>\<rho> \<rho>(x \<mapsto> \<lbrace>\<rbrace>)"
  apply (rule accept_value_accept_val_env.Any, auto)
       apply (erule accept_state_pool.cases, auto)
       apply (drule spec[of _ \<pi>])
@@ -823,9 +823,9 @@ lemma flow_over_pool_to_env_5: "
 done
 
 lemma flow_over_pool_to_stack_5: "
-  (\<V>, \<C>) \<Turnstile>\<^sub>\<E> \<E> \<Longrightarrow> \<E>' = \<E>(\<pi> ;; x \<mapsto> \<langle>e; \<rho>(x \<mapsto> \<lbrace>\<rbrace>); \<kappa>\<rangle>, \<pi>;;. \<mapsto> \<langle>e\<^sub>c; \<rho>; []\<rangle>) \<Longrightarrow> 
+  (\<V>, \<C>, \<X>) \<Turnstile>\<^sub>\<E> \<E> \<Longrightarrow> \<E>' = \<E>(\<pi> ;; x \<mapsto> \<langle>e; \<rho>(x \<mapsto> \<lbrace>\<rbrace>); \<kappa>\<rangle>, \<pi>;;. \<mapsto> \<langle>e\<^sub>c; \<rho>; []\<rangle>) \<Longrightarrow> 
   leaf \<E> \<pi> \<Longrightarrow> \<E> \<pi> = Some (\<langle>LET x = SPAWN e\<^sub>c in e; \<rho>; \<kappa>\<rangle>) \<Longrightarrow> 
-  (\<V>, \<C>) \<Turnstile>\<^sub>\<kappa>  \<V> (\<lfloor>e\<rfloor>) \<Rrightarrow> \<kappa>
+  (\<V>, \<C>, \<X>) \<Turnstile>\<^sub>\<kappa>  \<V> (\<lfloor>e\<rfloor>) \<Rrightarrow> \<kappa>
 "
  apply (erule accept_state_pool.cases, auto)
  apply (drule spec[of _ \<pi>])
@@ -834,9 +834,9 @@ lemma flow_over_pool_to_stack_5: "
 done
 
 lemma flow_over_pool_to_exp_6: "
-  (\<V>, \<C>) \<Turnstile>\<^sub>\<E> \<E> \<Longrightarrow> \<E>' = \<E>(\<pi> ;; x \<mapsto> \<langle>e; \<rho>(x \<mapsto> \<lbrace>\<rbrace>); \<kappa>\<rangle>, \<pi>;;. \<mapsto> \<langle>e\<^sub>c; \<rho>; []\<rangle>) \<Longrightarrow> 
+  (\<V>, \<C>, \<X>) \<Turnstile>\<^sub>\<E> \<E> \<Longrightarrow> \<E>' = \<E>(\<pi> ;; x \<mapsto> \<langle>e; \<rho>(x \<mapsto> \<lbrace>\<rbrace>); \<kappa>\<rangle>, \<pi>;;. \<mapsto> \<langle>e\<^sub>c; \<rho>; []\<rangle>) \<Longrightarrow> 
   leaf \<E> \<pi> \<Longrightarrow> \<E> \<pi> = Some (\<langle>LET x = SPAWN e\<^sub>c in e; \<rho>; \<kappa>\<rangle>) \<Longrightarrow> 
-  (\<V>, \<C>) \<Turnstile>\<^sub>e  e\<^sub>c
+  (\<V>, \<C>, \<X>) \<Turnstile>\<^sub>e  e\<^sub>c
 "   
  apply (erule accept_state_pool.cases, auto)
  apply (drule spec[of _ \<pi>])
@@ -846,9 +846,9 @@ lemma flow_over_pool_to_exp_6: "
 done
 
 lemma flow_over_pool_to_env_6: "
-  (\<V>, \<C>) \<Turnstile>\<^sub>\<E> \<E> \<Longrightarrow> \<E>' = \<E>(\<pi> ;; x \<mapsto> \<langle>e; \<rho>(x \<mapsto> \<lbrace>\<rbrace>); \<kappa>\<rangle>, \<pi>;;. \<mapsto> \<langle>e\<^sub>c; \<rho>; []\<rangle>) \<Longrightarrow> 
+  (\<V>, \<C>, \<X>) \<Turnstile>\<^sub>\<E> \<E> \<Longrightarrow> \<E>' = \<E>(\<pi> ;; x \<mapsto> \<langle>e; \<rho>(x \<mapsto> \<lbrace>\<rbrace>); \<kappa>\<rangle>, \<pi>;;. \<mapsto> \<langle>e\<^sub>c; \<rho>; []\<rangle>) \<Longrightarrow> 
   leaf \<E> \<pi> \<Longrightarrow> \<E> \<pi> = Some (\<langle>LET x = SPAWN e\<^sub>c in e; \<rho>; \<kappa>\<rangle>) \<Longrightarrow> 
-  (\<V>, \<C>) \<Turnstile>\<^sub>\<rho> \<rho>
+  (\<V>, \<C>, \<X>) \<Turnstile>\<^sub>\<rho> \<rho>
 "   
  apply (erule accept_state_pool.cases, auto)
  apply (drule spec[of _ \<pi>])
@@ -857,18 +857,18 @@ lemma flow_over_pool_to_env_6: "
 done
 
 lemma flow_over_pool_to_stack_6: "
-  (\<V>, \<C>) \<Turnstile>\<^sub>\<E> \<E> \<Longrightarrow> \<E>' = \<E>(\<pi> ;; x \<mapsto> \<langle>e; \<rho>(x \<mapsto> \<lbrace>\<rbrace>); \<kappa>\<rangle>, \<pi>;;. \<mapsto> \<langle>e\<^sub>c; \<rho>; []\<rangle>) \<Longrightarrow> 
+  (\<V>, \<C>, \<X>) \<Turnstile>\<^sub>\<E> \<E> \<Longrightarrow> \<E>' = \<E>(\<pi> ;; x \<mapsto> \<langle>e; \<rho>(x \<mapsto> \<lbrace>\<rbrace>); \<kappa>\<rangle>, \<pi>;;. \<mapsto> \<langle>e\<^sub>c; \<rho>; []\<rangle>) \<Longrightarrow> 
   leaf \<E> \<pi> \<Longrightarrow> \<E> \<pi> = Some (\<langle>LET x = SPAWN e\<^sub>c in e; \<rho>; \<kappa>\<rangle>) \<Longrightarrow> 
-  (\<V>, \<C>) \<Turnstile>\<^sub>\<kappa>  \<V> (\<lfloor>e\<^sub>c\<rfloor>) \<Rrightarrow> []
+  (\<V>, \<C>, \<X>) \<Turnstile>\<^sub>\<kappa>  \<V> (\<lfloor>e\<^sub>c\<rfloor>) \<Rrightarrow> []
 "   
  apply (rule accept_stack.Empty)
 done
 
 
 lemma flow_let_spawn_preservation: "
-  (\<V>, \<C>) \<Turnstile>\<^sub>\<E> \<E> \<Longrightarrow> \<E>' = \<E>(\<pi> ;; x \<mapsto> \<langle>e; \<rho>(x \<mapsto> \<lbrace>\<rbrace>); \<kappa>\<rangle>, \<pi>;;. \<mapsto> \<langle>e\<^sub>c; \<rho>; []\<rangle>) \<Longrightarrow>
+  (\<V>, \<C>, \<X>) \<Turnstile>\<^sub>\<E> \<E> \<Longrightarrow> \<E>' = \<E>(\<pi> ;; x \<mapsto> \<langle>e; \<rho>(x \<mapsto> \<lbrace>\<rbrace>); \<kappa>\<rangle>, \<pi>;;. \<mapsto> \<langle>e\<^sub>c; \<rho>; []\<rangle>) \<Longrightarrow>
   leaf \<E> \<pi> \<Longrightarrow> \<E> \<pi> = Some (\<langle>LET x = SPAWN e\<^sub>c in e; \<rho>; \<kappa>\<rangle>) \<Longrightarrow> 
-  (\<V>, \<C>) \<Turnstile>\<^sub>\<E> \<E>(\<pi> ;; x \<mapsto> \<langle>e; \<rho>(x \<mapsto> \<lbrace>\<rbrace>); \<kappa>\<rangle>, \<pi>;;. \<mapsto> \<langle>e\<^sub>c; \<rho>; []\<rangle>)
+  (\<V>, \<C>, \<X>) \<Turnstile>\<^sub>\<E> \<E>(\<pi> ;; x \<mapsto> \<langle>e; \<rho>(x \<mapsto> \<lbrace>\<rbrace>); \<kappa>\<rangle>, \<pi>;;. \<mapsto> \<langle>e\<^sub>c; \<rho>; []\<rangle>)
 "
   apply (rule accept_state_pool.Any, auto)
     apply (rule accept_state.Any)
@@ -885,10 +885,10 @@ done
 
 theorem flow_preservation : "
   \<lbrakk>
-    (\<V>, \<C>) \<Turnstile>\<^sub>\<E> \<E>; 
+    (\<V>, \<C>, \<X>) \<Turnstile>\<^sub>\<E> \<E>; 
     \<E> \<rightarrow> \<E>'
   \<rbrakk> \<Longrightarrow>
-  (\<V>, \<C>) \<Turnstile>\<^sub>\<E> \<E>'
+  (\<V>, \<C>, \<X>) \<Turnstile>\<^sub>\<E> \<E>'
 "
  apply (erule concur_step.cases, auto)
     apply (erule flow_seq_step_preservation, auto)
@@ -899,9 +899,8 @@ done
 
 theorem flow_preservation_star' : "
   \<E> \<rightarrow>* \<E>' \<Longrightarrow>
-  ((\<V>, \<C>) \<Turnstile>\<^sub>\<E> \<E> \<longrightarrow> (\<V>, \<C>) \<Turnstile>\<^sub>\<E> \<E>')
+  ((\<V>, \<C>, \<X>) \<Turnstile>\<^sub>\<E> \<E> \<longrightarrow> (\<V>, \<C>, \<X>) \<Turnstile>\<^sub>\<E> \<E>')
 "
- thm star.induct[of concur_step]
  apply (erule star.induct[of concur_step], auto)
  apply (rename_tac \<E> \<E>' \<E>'')
  apply (erule notE)
@@ -911,15 +910,15 @@ done
 
 theorem flow_preservation_star : "
   \<lbrakk>
-    (\<V>, \<C>) \<Turnstile>\<^sub>\<E> \<E>;  
+    (\<V>, \<C>, \<X>) \<Turnstile>\<^sub>\<E> \<E>;  
     \<E> \<rightarrow>* \<E>'
   \<rbrakk> \<Longrightarrow>
-  (\<V>, \<C>) \<Turnstile>\<^sub>\<E> \<E>'
+  (\<V>, \<C>, \<X>) \<Turnstile>\<^sub>\<E> \<E>'
 "
 by (drule flow_preservation_star', auto)
 
 theorem flow_over_env_precision : "
-  (\<V>, \<C>) \<Turnstile>\<^sub>\<rho> \<rho>
+  (\<V>, \<C>, \<X>) \<Turnstile>\<^sub>\<rho> \<rho>
   \<Longrightarrow>
   \<parallel>\<rho>\<parallel> \<sqsubseteq> \<V>
 "
@@ -930,7 +929,7 @@ theorem flow_over_env_precision : "
 done
 
 theorem flow_over_state_precision : "
-  (\<V>, \<C>) \<Turnstile>\<^sub>\<sigma> \<langle>e; \<rho>; \<kappa>\<rangle>
+  (\<V>, \<C>, \<X>) \<Turnstile>\<^sub>\<sigma> \<langle>e; \<rho>; \<kappa>\<rangle>
   \<Longrightarrow>
   \<parallel>\<rho>\<parallel> \<sqsubseteq> \<V>
 "
@@ -940,11 +939,11 @@ done
 
 lemma flow_over_pool_to_state: "
   \<lbrakk>
-    (\<V>, \<C>) \<Turnstile>\<^sub>\<E> \<E>; 
+    (\<V>, \<C>, \<X>) \<Turnstile>\<^sub>\<E> \<E>; 
     \<E> \<pi> = Some \<sigma> 
   \<rbrakk>
   \<Longrightarrow>
-  (\<V>, \<C>) \<Turnstile>\<^sub>\<sigma>  \<sigma>
+  (\<V>, \<C>, \<X>) \<Turnstile>\<^sub>\<sigma>  \<sigma>
 "
  apply (erule accept_state_pool.cases)
  apply (drule spec[of _ \<pi>])
@@ -954,7 +953,7 @@ done
   
 theorem flow_over_pool_precision : "
   \<lbrakk>
-    (\<V>, \<C>) \<Turnstile>\<^sub>\<E> \<E>;
+    (\<V>, \<C>, \<X>) \<Turnstile>\<^sub>\<E> \<E>;
     \<E> \<pi> = Some (\<langle>e; \<rho>; \<kappa>\<rangle>)
   \<rbrakk>
   \<Longrightarrow>
@@ -964,44 +963,98 @@ theorem flow_over_pool_precision : "
  apply (erule flow_over_state_precision)
 done
 
-theorem lift_flow_exp_to_state: "(\<V>, \<C>) \<Turnstile>\<^sub>e e \<Longrightarrow> (\<V>, \<C>) \<Turnstile>\<^sub>\<sigma>  \<langle>e; empty; []\<rangle>"
+theorem lift_flow_exp_to_state: "(\<V>, \<C>, \<X>) \<Turnstile>\<^sub>e e \<Longrightarrow> (\<V>, \<C>, \<X>) \<Turnstile>\<^sub>\<sigma>  \<langle>e; empty; []\<rangle>"
  apply (rule accept_state.Any, auto)
  apply (rule+, auto, rule)
 done
 
-theorem  lift_flow_state_to_pool: "(\<V>, \<C>) \<Turnstile>\<^sub>\<sigma>  \<sigma> \<Longrightarrow> (\<V>, \<C>) \<Turnstile>\<^sub>\<E> [[] \<mapsto> \<sigma>]"
+theorem  lift_flow_state_to_pool: "(\<V>, \<C>, \<X>) \<Turnstile>\<^sub>\<sigma>  \<sigma> \<Longrightarrow> (\<V>, \<C>, \<X>) \<Turnstile>\<^sub>\<E> [[] \<mapsto> \<sigma>]"
   apply (rule accept_state_pool.Any)
   apply (case_tac "\<pi> = []", auto)
 done
 
-theorem lift_flow_exp_to_pool: "(\<V>, \<C>) \<Turnstile>\<^sub>e  e \<Longrightarrow> (\<V>, \<C>) \<Turnstile>\<^sub>\<E> [[] \<mapsto> \<langle>e; empty; []\<rangle>]"
+theorem lift_flow_exp_to_pool: "(\<V>, \<C>, \<X>) \<Turnstile>\<^sub>e  e \<Longrightarrow> (\<V>, \<C>, \<X>) \<Turnstile>\<^sub>\<E> [[] \<mapsto> \<langle>e; empty; []\<rangle>]"
   apply (drule lift_flow_exp_to_state)
   apply (erule lift_flow_state_to_pool)
 done
 
 theorem flow_over_pool_sound : "
   \<lbrakk>
-    (\<V>, \<C>) \<Turnstile>\<^sub>\<E> \<E>; 
+    (\<V>, \<C>, \<X>) \<Turnstile>\<^sub>\<E> \<E>; 
     \<E> \<rightarrow>* \<E>';
     \<E>' \<pi> = Some (\<langle>e'; \<rho>'; \<kappa>'\<rangle>)
   \<rbrakk> \<Longrightarrow>
   \<parallel>\<rho>'\<parallel> \<sqsubseteq> \<V>
 "
- apply (drule flow_preservation_star [of \<V> \<C> _ \<E>'], auto)
- apply (erule flow_over_pool_precision [of \<V> \<C> \<E>' \<pi> e' \<rho>' \<kappa>'], auto)
+ apply (drule flow_preservation_star [of \<V> \<C> \<X> _ \<E>'], auto)
+ apply (erule flow_over_pool_precision [of \<V> \<C> \<X> \<E>' \<pi> e' \<rho>' \<kappa>'], auto)
 done
 
 
 theorem flow_sound : "
   \<lbrakk>
-    (\<V>, \<C>) \<Turnstile>\<^sub>e  e; 
+    (\<V>, \<C>, \<X>) \<Turnstile>\<^sub>e e; 
     [[] \<mapsto> \<langle>e; empty; []\<rangle>] \<rightarrow>* \<E>';
     \<E>' \<pi> = Some (\<langle>e'; \<rho>'; \<kappa>'\<rangle>)
   \<rbrakk> \<Longrightarrow>
   \<parallel>\<rho>'\<parallel> \<sqsubseteq> \<V>
 "
  apply (drule lift_flow_exp_to_pool)
- apply (erule flow_over_pool_sound [of \<V> \<C> _ \<E>' \<pi> e' \<rho>' \<kappa>'], auto)
+ apply (erule flow_over_pool_sound [of \<V> \<C> \<X> _ \<E>' \<pi> e' \<rho>' \<kappa>'], auto)
+done
+
+corollary flow_sound_coro: "
+  \<lbrakk>
+    (\<V>, \<C>, \<X>) \<Turnstile>\<^sub>e e ;
+    [[] \<mapsto> \<langle>e;Map.empty;[]\<rangle>] \<rightarrow>* \<E>';
+    \<E>' \<pi> = Some (\<langle>e';\<rho>';\<kappa>'\<rangle>);
+    \<rho>' x = Some \<omega>
+  \<rbrakk> \<Longrightarrow>
+  {|\<omega>|} \<subseteq> \<V> x
+"
+  apply (drule flow_sound; assumption?)
+  apply (unfold abstract_value_env_precision_def)
+  apply (unfold env_to_abstract_value_env_def)
+  apply (drule spec[of _ x]; auto)
+done
+
+(*****)
+
+theorem bind_flow_over_pool_precision : "
+  \<lbrakk>
+    (\<V>, \<C>, \<X>) \<Turnstile>\<^sub>\<E> \<E>;
+    \<E> \<pi> = Some (\<langle>LET x = b in e; \<rho>; \<kappa>\<rangle>)
+  \<rbrakk>
+  \<Longrightarrow>
+  {b} \<subseteq> \<X> x
+"
+ apply (drule flow_over_pool_to_state, simp)
+ apply  (erule accept_state.cases; auto)
+ apply  (erule accept_exp.cases; auto)
+done
+
+theorem bind_flow_over_pool_sound : "
+  \<lbrakk>
+    (\<V>, \<C>, \<X>) \<Turnstile>\<^sub>\<E> \<E>; 
+    \<E> \<rightarrow>* \<E>';
+    \<E>' \<pi> = Some (\<langle>LET x' = b' in e'; \<rho>'; \<kappa>'\<rangle>)
+  \<rbrakk> \<Longrightarrow>
+  {b'} \<subseteq> \<X> x'
+"
+ apply (drule flow_preservation_star [of \<V> \<C> \<X> _ \<E>'], auto)
+ apply (drule bind_flow_over_pool_precision, auto)
+done
+
+theorem bind_flow_sound : "
+  \<lbrakk>
+    (\<V>, \<C>, \<X>) \<Turnstile>\<^sub>e e; 
+    [[] \<mapsto> \<langle>e; empty; []\<rangle>] \<rightarrow>* \<E>';
+    \<E>' \<pi> = Some (\<langle>LET x' = b' in e'; \<rho>'; \<kappa>'\<rangle>)
+  \<rbrakk> \<Longrightarrow>
+  {b'} \<subseteq> \<X> x'
+"
+ apply (drule lift_flow_exp_to_pool)
+ apply (erule bind_flow_over_pool_sound[of _ _ _ "[[] \<mapsto> \<langle>e; empty; []\<rangle>]" \<E>' \<pi>]; auto)
 done
 
 end
