Semantics.thy
@@ -24,7 +24,7 @@ type_synonym state_pool = "control_path \<rightharpoonup> state"
 inductive seq_step :: "state \<Rightarrow> state \<Rightarrow> bool" (infix "\<hookrightarrow>" 55) where 
   Result: "
     \<rho> x = Some \<omega> \<Longrightarrow>
-    \<langle>RESULT x; \<rho>; \<langle>x\<^sub>\<kappa>, e\<^sub>\<kappa>, \<rho>\<^sub>\<kappa>\<rangle> # \<kappa>\<rangle>\<hookrightarrow> \<langle>e\<^sub>\<kappa>; \<rho>\<^sub>\<kappa> ++ [x\<^sub>\<kappa> \<mapsto> \<omega>]; \<kappa>\<rangle>
+    \<langle>RESULT x; \<rho>; \<langle>x\<^sub>\<kappa>, e\<^sub>\<kappa>, \<rho>\<^sub>\<kappa>\<rangle> # \<kappa>\<rangle> \<hookrightarrow> \<langle>e\<^sub>\<kappa>; \<rho>\<^sub>\<kappa> ++ [x\<^sub>\<kappa> \<mapsto> \<omega>]; \<kappa>\<rangle>
   " |
   Let_Unit: "
     \<langle>LET x = \<lparr>\<rparr> in e; \<rho>; \<kappa>\<rangle> \<hookrightarrow> \<langle>e; \<rho> ++ [x \<mapsto> \<lbrace>\<rbrace>]; \<kappa>\<rangle>
